.fst for monotonic buffers

ulib/LowStar.Monotonic.Buffer.fst
@@ -8,27 +8,12 @@ module Seq = FStar.Seq
 module HS = FStar.HyperStack
 module HST = FStar.HyperStack.ST
 
-(* Most comments are taken from the Low* tutorial at:
-   https://fstarlang.github.io/lowstar/html/LowStar.html
- *)
-
-/// Low* buffers
-/// ==============
-///
-/// The workhorse of Low*, this module allows modeling C arrays on the
-/// stack and in the heap.  At compilation time, KreMLin implements
-/// buffers using C arrays, i.e. if Low* type ``t`` is translated into C
-/// type ``u``, then Low* type ``buffer t`` is translated to C type ``u*``.
-
-(*
- * Replacing subsequence in s at (offset, offset + len) by sub
- *)
-let replace_subseq (#a:Type0)
+private let replace_subseq (#a:Type0)
   (s:Seq.seq a) (offset:nat) (len:nat{offset + len <= Seq.length s}) (sub:Seq.lseq a len)
   :Tot (Seq.seq a)
-  = Seq.append (Seq.slice s 0 offset) (Seq.append sub (Seq.slice s (offset + len) (Seq.length s)))
+  = Seq.replace_subseq s offset (offset + len) sub
 
-let lemma_replace_subseq_elim (#a:Type0)
+private let lemma_replace_subseq_elim (#a:Type0)
   (s:Seq.seq a) (offset:nat) (len:nat{offset + len <= Seq.length s}) (sub:Seq.lseq a len)
   :Lemma (let s1 = replace_subseq s offset len sub in
           Seq.length s1 == Seq.length s /\
@@ -38,431 +23,94 @@ let lemma_replace_subseq_elim (#a:Type0)
 	 [SMTPat (replace_subseq s offset len sub)]
   = ()
 
-(*
- * Shorthand slice, that takes length as the second argument
- *)
-private let mslice (#a:Type0) (s:Seq.seq a) (offset:nat) (len:nat{offset + len <= Seq.length s}) :Tot (Seq.seq a) =
-  Seq.slice s offset (offset + len)
-
-(* Shorthand for preorder over sequences *)
-type srel (a:Type0) = P.preorder (Seq.seq a)
-
 private let srel_to_lsrel (#a:Type0) (len:nat) (pre:srel a) :P.preorder (Seq.lseq a len) = fun s1 s2 -> pre s1 s2
 
-(*
- * Notion of compatibility for the preorders on subbuffers
- *
- * The compatibility is both ways implication
- *   (a) When the parent sequence changes according to its preorder,
- *       the subsequence (offset, offset + len) should respect the sub preorder
- *   (b) When the subsequence (offset, offset + len) changed accoring to the sub preorder,
- *       the replace_subseq in the parent sequence should respect its preorder
- *
- * The direction (b) is required for valid updates
- *   In the sense that clients will update the buffer according to the buffer preorder,
- *   And since this will result in an update in the underlying reference, we need the direction (b)
- *
- * Where will the direction (a) be required? My guess is, when witnessing predicates on the buffer preorder
- *   Again, clients will witness according to the buffer preorder,
- *   And this will result in witness on the underlying reference, so we would need the direction (a)
- *)
-let compatible_sub_preorder (#a:Type0)
-  (len:nat) (pre:srel a)
-  (offset:nat) (sub_len:nat{offset + sub_len <= len}) (sub_pre:srel a)
-  = (forall (s1 s2:Seq.seq a). (Seq.length s1 == len /\ Seq.length s2 == len /\ pre s1 s2) ==>
-		          (sub_pre (mslice s1 offset sub_len) (mslice s2 offset sub_len))) /\  //(a)
-    (forall (s s2:Seq.seq a). (Seq.length s == len /\ Seq.length s2 == sub_len /\ sub_pre (mslice s offset sub_len) s2) ==>
-  		         (pre s (replace_subseq s offset sub_len s2)))  //(b)
-
-(*
- * Reflexivity of the compatibility relation
- *)
-let lemma_sub_compatilibity_is_reflexive (#a:Type0) (len:nat) (pre:srel a)
-  :Lemma (compatible_sub_preorder len pre 0 len pre)
-  = assert (forall (s1 s2:Seq.seq a). Seq.length s1 == Seq.length s2 ==>
-                                 Seq.equal (replace_subseq s1 0 (Seq.length s1) s2) s2)
-
-(*
- * Transitivity of the compatibility relation
- *)
-let lemma_sub_compatibility_is_transitive (#a:Type0)
-  (len:nat) (pre:srel a)
-  (offset1 len1:nat) (pre1:srel a)
-  (offset2 len2:nat) (pre2:srel a)
-  :Lemma (requires (offset1 + len1 <= len /\ offset2 + len2 <= len1 /\
-                    compatible_sub_preorder len pre offset1 len1 pre1 /\
-                    compatible_sub_preorder len1 pre1 offset2 len2 pre2))
-	 (ensures  (compatible_sub_preorder len pre (offset1 + offset2) len2 pre2))
-  = admit () (*
- * Key lemma to prove the transitivity of the compatibility relation (to come later)
- * The lemma says that replace_subseq commutes with slice
- * We can either
- *  (a) Replace a subsequence in s at (offset1 + offset2, offset1 + offset2 + len2) by s2, OR
- *  (b) Take the slice of s at (offset1, offset1 + len1),
-        replace subsequence in the slice at (offset2, offset2 + len2),
-	and then replace the subsequence in s at (offset1, offset1 + len1) with this updated slice
- * Both give us the same sequence
- *)
-// private let lemma_replace_subseq_slice
-//   (a:Type0) (len offset1 len1 offset2 len2:nat)
-//   (s:Seq.lseq a len) (s2:Seq.lseq a len2)
-//   :Lemma ((offset1 + len1 <= len /\ offset2 + len2 <= len1) ==>
-// 	  (Seq.equal (replace_subseq s (offset1 + offset2) len2 s2)
-// 	             (replace_subseq s offset1 len1 (replace_subseq (mslice s offset1 len1)
-// 						                    offset2 len2 s2))))
-//   = ()
-
- 
-  
-//   Classical.forall_intro_2 (lemma_replace_subseq_slice a len offset1 len1 offset2 len2)
-
-(*
- * The type is indexed by two preorders:
- *   rrel: is the preorder of the underlying reference
- *   rel : is the preorder of the buffer itself
-  * It is less than ideal to keep rrel in the index :(
- * But hiding it in the inductive bumps up the universe to Type u#1
- *   which means no buffers of buffers
- * Hopefully we can build libraries over it so that rarely will clients need to use mbuffer a rrel rel
- *)
-abstract noeq type mbuffer (a:Type0) (rrel:srel a) (rel:srel a) :Type0 =
+noeq type mbuffer (a:Type0) (rrel:srel a) (rel:srel a) :Type0 =
   | Null
   | Buffer:
-    max_length: U32.t ->
-    content: HST.mreference (Seq.lseq a (U32.v max_length)) (srel_to_lsrel (U32.v max_length) rrel) ->
-    idx: U32.t ->
-    length: U32.t{U32.v idx + U32.v length <= U32.v max_length} ->
-    compatible: squash (compatible_sub_preorder (U32.v max_length) rrel
-                                                (U32.v idx) (U32.v length) rel) ->  //proof of compatibility
+    max_length:U32.t ->
+    content:HST.mreference (Seq.lseq a (U32.v max_length)) (srel_to_lsrel (U32.v max_length) rrel) ->
+    idx:U32.t ->
+    length:U32.t{U32.v idx + U32.v length <= U32.v max_length} ->
+    compatible:squash (Seq.compatible_sub_preorder (U32.v max_length) rrel
+                                                    (U32.v idx) (U32.v idx + U32.v length) rel) ->  //proof of compatibility
     mbuffer a rrel rel
 
-/// The C ``NULL`` pointer is represented as the Low* ``null`` buffer. For
-/// any given type, there is exactly one ``null`` buffer of this type,
-/// just like there is exactly one C ``NULL`` pointer of any given type.
-///
-/// The nullity test ``g_is_null`` is ghost, for proof purposes
-/// only. The corresponding stateful nullity test is ``is_null``, see
-/// below.
-
-(* FIXME: The nullity test for proof purposes is currently expressed
-   as a ghost predicate, `g_is_null`, but it is scheduled to be
-   replaced with equality with `null` *)
-
-abstract val g_is_null (#a:Type0) (#rrel:srel a) (#rel:srel a) (b:mbuffer a rrel rel) :GTot bool
 let g_is_null #_ #_ #_ b = Null? b
 
-abstract val null (#a:Type0) (#rrel:srel a) (#rel:srel a) :Tot (b:mbuffer a rrel rel {g_is_null b})
 let null #_ #_ #_ = Null
 
-abstract val null_unique (#a:Type0) (#rrel:srel a) (#rel:srel a) (b:mbuffer a rrel rel)
-  :Lemma (g_is_null b <==> b == null)
 let null_unique #_ #_ #_ _ = ()
 
-/// ``unused_in b h`` holds only if buffer ``b`` has not been allocated
-/// yet.
-
-abstract val unused_in (#a:Type0) (#rrel:srel a) (#rel:srel a) (b:mbuffer a rrel rel) (h:HS.mem) :GTot Type0
 let unused_in #_ #_ #_ b h =
   match b with
   | Null -> False
   | Buffer _ content _ _ _ -> content `HS.unused_in` h
 
-/// ``live h b`` holds if, and only if, buffer ``b`` is currently
-/// allocated in ``h`` and has not been deallocated yet.
-///
-/// This predicate corresponds to the C notion of "lifetime", and as
-/// such, is a prerequisite for all stateful operations on buffers
-/// (see below), per the C standard:
-///
-///   If an object is referred to outside of its lifetime, the
-///   behavior is undefined.
-/// 
-///   -- ISO/IEC 9899:2011, Section 6.2.4 paragraph 2
-/// 
-/// By contrast, it is not required for the ghost versions of those
-/// operators.
-
-abstract val live (#a:Type0) (#rrel:srel a) (#rel:srel a) (h:HS.mem) (b:mbuffer a rrel rel) :GTot Type0
 let live #_ #_ #_ h b =
   match b with
   | Null -> True
   | Buffer _ content _ _ _ -> h `HS.contains` content
 
-/// The null pointer is always live.
+let live_null _ _ _ _ = ()
 
-abstract val live_null (a:Type0) (#rrel:srel a) (#rel:srel a) (h:HS.mem)  (* TODO: make a wrapper for default preorders *)
-  :Lemma (live h (null #a #rrel #rel))
-let live_null a #_ #_ h = ()
-
-let live_is_null (#a:Type0) (#rrel:srel a) (#rel:srel a) (h:HS.mem) (b:mbuffer a rrel rel)
-  :Lemma (requires (g_is_null b == true))
-         (ensures (live h b))
-         [SMTPat (live h b)]
-  = null_unique b;
-    live_null a #rrel #rel h
-
-
-/// A live buffer has already been allocated.
-
-abstract val live_not_unused_in (#a:Type0) (#rrel:srel a) (#rel:srel a) (h:HS.mem) (b:mbuffer a rrel rel)
-  :Lemma (requires (live h b /\ b `unused_in` h))
-         (ensures False)
 let live_not_unused_in #_ #_ #_ _ _ = ()
 
-(* FIXME: the following definition is necessary to isolate the pattern
-   because of unification. In other words, if we attached the pattern
-   to `live_not_unused_in`, then we would not be able to use
-   `FStar.Classical.forall_intro_`n and
-   `FStar.Classical.move_requires` due to unification issues.  Anyway,
-   we plan to isolate patterns in a separate module to clean up the Z3
-   context.
- *)
-
-let live_not_unused_in' (#a:Type0) (#rrel:srel a) (#rel:srel a) (h:HS.mem) (b:mbuffer a rrel rel)
-  :Lemma (requires (live h b /\ b `unused_in` h))
-         (ensures False)
-         [SMTPat (live h b); SMTPat (b `unused_in` h)]
-  = live_not_unused_in h b
-
-
-/// Buffers live in the HyperStack model, which is an extension of
-/// the HyperHeap model, a hierarchical memory model that divides the
-/// heap into a tree of regions. This coarse-grained separation
-/// allows the programmer to state modifies clauses at the level of
-/// regions, rather than on individual buffers.
-///
-/// The HyperHeap memory model is described:
-///  - in the 2016 POPL paper: https://www.fstar-lang.org/papers/mumon/
-///  - in the relevant section of the F* tutorial: http://www.fstar-lang.org/tutorial/
-///
-/// ``frameOf b`` returns the identifier of the region in which the
-/// buffer ``b`` lives.
-
-abstract val frameOf (#a:Type0) (#rrel:srel a) (#rel:srel a) (b:mbuffer a rrel rel) :Tot HS.rid
 let frameOf #_ #_ #_ b = if Null? b then HS.root else HS.frameOf (Buffer?.content b)
 
-
-/// ``as_addr b`` returns the abstract address of the buffer in its
-/// region, as an allocation unit: two buffers that are allocated
-/// separately in the same region will actually have different
-/// addresses, but a sub-buffer of a buffer will actually have the
-/// same address as its enclosing buffer.
-
-abstract val as_addr (#a:Type0) (#rrel:srel a) (#rel:srel a) (b:mbuffer a rrel rel) :GTot nat
 let as_addr #_ #_ #_  b = if g_is_null b then 0 else HS.as_addr (Buffer?.content b)
 
-
-/// A buffer is unused if, and only if, its address is unused.
-
-abstract val unused_in_equiv (#a:Type0) (#rrel:srel a) (#rel:srel a) (b:mbuffer a rrel rel) (h:HS.mem)
-  :Lemma (unused_in b h <==>
-          (HS.live_region h (frameOf b) ==> as_addr b `Heap.addr_unused_in` (Map.sel (HS.get_hmap h) (frameOf b))))
 let unused_in_equiv #_ #_ #_ b h =
   if g_is_null b then Heap.not_addr_unused_in_nullptr (Map.sel (HS.get_hmap h) HS.root) else ()
 
-
-/// If a buffer is live, then so is its region.
-
-abstract val live_region_frameOf (#a:Type0) (#rrel:srel a) (#rel:srel a) (h:HS.mem) (b:mbuffer a rrel rel)
-  :Lemma (requires (live h b))
-         (ensures (HS.live_region h (frameOf b)))
-         [SMTPatOr [
-	   [SMTPat (live h b)];
-           [SMTPat (HS.live_region h (frameOf b))];
-         ]]
 let live_region_frameOf #_ #_ #_ _ _ = ()
 
-
-/// The length of a buffer ``b`` is available as a machine integer ``len
-/// b`` or as a mathematical integer ``length b``, but both in ghost
-/// (proof) code only: just like in C, one cannot compute the length
-/// of a buffer at run-time.
-
-abstract val len (#a:Type0) (#rrel:srel a) (#rel:srel a) (b:mbuffer a rrel rel) :GTot U32.t
 let len #_ #_ #_ b =
   match b with
   | Null -> 0ul
   | Buffer _ _ _ len _ -> len
 
-let length (#a:Type0) (#rrel:srel a) (#rel:srel a) (b:mbuffer a rrel rel) :GTot nat = U32.v (len b)
+let len_null a _ _ = ()
 
-
-/// The null pointer has length 0.
-
-abstract val len_null (a:Type0) (#rrel:srel a) (#rel:srel a)  (* TODO: add a wrapper for default preorder *)
-  :Lemma (len (null #a #rrel #rel) == 0ul)
-let len_null a #_ #_ = ()
-
-let length_null_1 (#a:Type0) (#rrel:srel a) (#rel:srel a) (b:mbuffer a rrel rel)
-  :Lemma (requires (length b =!= 0)) (ensures (g_is_null b == false))
-         [SMTPat (length b)]
-  = len_null a #rrel #rel;
-    null_unique b
-
-let length_null_2 (#a:Type0) (#rrel:srel a) (#rel:srel a) (b:mbuffer a rrel rel)
-  :Lemma (requires (g_is_null b == true)) (ensures (length b == 0))
-         [SMTPat (g_is_null b)]
-  = len_null a #rrel #rel;
-    null_unique b
-
-
-/// For functional correctness, buffers are reflected at the proof
-/// level using sequences, via ``as_seq b h``, which returns the
-/// contents of a given buffer ``b`` in a given heap ``h``. If ``b`` is not
-/// live in ``h``, then the result is unspecified.
-
-(* TODO: why not return a lseq and remove length_as_seq lemma? *)
-abstract val as_seq (#a:Type0) (#rrel:srel a) (#rel:srel a) (h:HS.mem) (b:mbuffer a rrel rel) :GTot (Seq.seq a)
 let as_seq #_ #_ #_ h b =
   match b with
   | Null -> Seq.empty
   | Buffer max_len content idx len _ ->
     Seq.slice (HS.sel h content) (U32.v idx) (U32.v idx + U32.v len)
 
-/// The contents of a buffer ``b`` has the same length as ``b`` itself.
-
-abstract val length_as_seq (#a:Type0) (#rrel:srel a) (#rel:srel a) (h:HS.mem) (b:mbuffer a rrel rel)
-  :Lemma (Seq.length (as_seq h b) == length b)
-         [SMTPat (Seq.length (as_seq h b))]
 let length_as_seq #_ #_ #_ _ _ = ()
 
-
-/// ``get`` is an often-convenient shorthand to index the value of a
-/// given buffer in a given heap, for proof purposes.
-
-let get (#a:Type0) (#rrel:srel a) (#rel:srel a) (h:HS.mem) (p:mbuffer a rrel rel) (i:nat)
-  :Ghost a (requires (i < length p)) (ensures (fun _ -> True))
-  = Seq.index (as_seq h p) i
-
-
-/// ``gsub`` is the way to carve a sub-buffer out of a given
-/// buffer. ``gsub b i len`` return the sub-buffer of ``b`` starting from
-/// offset ``i`` within ``b``, and with length ``len``. Of course ``i`` and
-/// ``len`` must fit within the length of ``b``.
-///
-/// Clients can provide a preorder at which they want to take the subbuffer
-/// But they have to prove compatibility
-///
-/// ``gsub`` is the ghost version, for proof purposes. Its stateful
-/// counterpart is ``sub``, see below.
-
-unfold let compatible_sub
-  (#a:Type0) (#rrel:srel a) (#rel:srel a)
-  (b:mbuffer a rrel rel) (i:U32.t) (len:U32.t{U32.v i + U32.v len <= length b}) (sub_rel:srel a)
-  = compatible_sub_preorder (length b) rel (U32.v i) (U32.v len) sub_rel
-
-(*
- * TODO: candidate for writing a wrapper
- *       also now there is a compatibility query for each of the gsub operation
- *       would it be worth writing a wrapper for each of those functions?
- *)
-abstract val gsub (#a:Type0) (#rrel:srel a) (#rel:srel a) 
-  (b:mbuffer a rrel rel) (i:U32.t) (len:U32.t) (sub_rel:srel a)
-  : Ghost (mbuffer a rrel sub_rel)
-          (requires (U32.v i + U32.v len <= length b /\
-	             compatible_sub b i len sub_rel))
-	  (ensures (fun _ -> True))
 let gsub #a #rrel #rel b i len sub_rel =
   match b with
   | Null -> Null
   | Buffer max_len content idx length () ->
-    lemma_sub_compatibility_is_transitive (U32.v max_len) rrel
-                                          (U32.v idx) (U32.v length) rel
-					  (U32.v i) (U32.v len) sub_rel;
+    Seq.lemma_seq_sub_compatibility_is_transitive (U32.v max_len) rrel
+                                                  (U32.v idx) (U32.v idx + U32.v length) rel
+		         			  (U32.v i) (U32.v i + U32.v len) sub_rel;
     Buffer max_len content (U32.add idx i) len ()
 
-// goffset
-
-/// A buffer is live exactly at the same time as all of its sub-buffers.
-
-abstract val live_gsub (#a:Type0) (#rrel:srel a) (#rel:srel a)
-  (h:HS.mem) (b:mbuffer a rrel rel) (i:U32.t) (len:U32.t) (sub_rel:srel a)
-  :Lemma (requires (U32.v i + U32.v len <= length b /\ compatible_sub b i len sub_rel))
-         (ensures  (live h (gsub b i len sub_rel) <==> live h b))
-         [SMTPatOr [
-             [SMTPat (live h (gsub b i len sub_rel))];
-             [SMTPat (live h b); SMTPat (gsub b i len sub_rel);]
-         ]]
 let live_gsub #_ #_ #_ _ _ _ _ _ = ()
 
-abstract val gsub_is_null (#a:Type0) (#rrel:srel a) (#rel:srel a)
-  (b:mbuffer a rrel rel) (i:U32.t) (len:U32.t) (sub_rel:srel a)
-  :Lemma (requires (U32.v i + U32.v len <= length b /\ compatible_sub b i len sub_rel))
-         (ensures (g_is_null (gsub b i len sub_rel) <==> g_is_null b))
-         [SMTPat (g_is_null (gsub b i len sub_rel))]
 let gsub_is_null #_ #_ #_ _ _ _ _ = ()
 
-
-/// The length of a sub-buffer is exactly the one provided at ``gsub``.
-
-abstract val len_gsub (#a:Type0) (#rrel:srel a) (#rel:srel a)
-  (b:mbuffer a rrel rel) (i:U32.t) (len':U32.t) (sub_rel:srel a)
-  :Lemma (requires (U32.v i + U32.v len' <= length b /\ compatible_sub b i len' sub_rel))
-         (ensures (len (gsub b i len' sub_rel) == len'))
-         [SMTPatOr [
-             [SMTPat (len (gsub b i len' sub_rel))];
-             [SMTPat (length (gsub b i len' sub_rel))];
-         ]]
 let len_gsub #_ #_ #_ _ _ _ _ = ()
 
-abstract val frameOf_gsub (#a:Type0) (#rrel:srel a) (#rel:srel a)
-  (b:mbuffer a rrel rel) (i:U32.t) (len:U32.t) (sub_rel:srel a)
-  :Lemma (requires (U32.v i + U32.v len <= length b /\ compatible_sub b i len sub_rel))
-         (ensures (frameOf (gsub b i len sub_rel) == frameOf b))
-  [SMTPat (frameOf (gsub b i len sub_rel))]
 let frameOf_gsub #_ #_ #_ _ _ _ _ = ()
 
-abstract val as_addr_gsub (#a:Type0) (#rrel:srel a) (#rel:srel a)
-  (b:mbuffer a rrel rel) (i:U32.t) (len:U32.t) (sub_rel:srel a)
-  :Lemma (requires (U32.v i + U32.v len <= length b /\ compatible_sub b i len sub_rel))
-         (ensures (as_addr (gsub b i len sub_rel) == as_addr b))
-         [SMTPat (as_addr (gsub b i len sub_rel))]
 let as_addr_gsub #_ #_ #_ _ _ _ _ = ()
 
-(* TODO: candidate for writing a wrapper *)
-abstract val gsub_inj (#a:Type0) (#rrel:srel a) (#rel:srel a)
-  (b1 b2:mbuffer a rrel rel)
-  (i1 i2:U32.t)
-  (len1 len2:U32.t)
-  (sub_rel1 sub_rel2:srel a)
-  :Lemma (requires (U32.v i1 + U32.v len1 <= length b1 /\ compatible_sub b1 i1 len1 sub_rel1 /\
-                    U32.v i2 + U32.v len2 <= length b2 /\ compatible_sub b2 i2 len2 sub_rel2 /\
-		    gsub b1 i1 len1 sub_rel1 === gsub b2 i2 len2 sub_rel2))
-         (ensures (len1 == len2 /\ (b1 == b2 ==> i1 == i2) /\ ((i1 == i2 /\ length b1 == length b2) ==> b1 == b2)))
 let gsub_inj #_ #_ #_ _ _ _ _ _ _ _ _ = ()
 
-
-/// Nesting two ``gsub`` collapses into one ``gsub``, transitively.
-
-abstract val gsub_gsub (#a:Type0) (#rrel:srel a) (#rel:srel a)
-  (b:mbuffer a rrel rel)
-  (i1:U32.t) (len1:U32.t) (sub_rel1:srel a)
-  (i2: U32.t) (len2: U32.t) (sub_rel2:srel a)
-  :Lemma (requires (U32.v i1 + U32.v len1 <= length b /\ compatible_sub b i1 len1 sub_rel1 /\
-                    U32.v i2 + U32.v len2 <= U32.v len1 /\ compatible_sub (gsub b i1 len1 sub_rel1) i2 len2 sub_rel2))
-         (ensures  (compatible_sub b (U32.add i1 i2) len2 sub_rel2 /\
-                    gsub (gsub b i1 len1 sub_rel1) i2 len2 sub_rel2 == gsub b (U32.add i1 i2) len2 sub_rel2))
-         [SMTPat (gsub (gsub b i1 len1 sub_rel1) i2 len2 sub_rel2)]
 let gsub_gsub #_ #_ #rel b i1 len1 sub_rel1 i2 len2 sub_rel2 =
-  lemma_sub_compatibility_is_transitive (length b) rel (U32.v i1) (U32.v len1) sub_rel1 (U32.v i2) (U32.v len2) sub_rel2
+  Seq.lemma_seq_sub_compatibility_is_transitive (length b) rel (U32.v i1) (U32.v i1 + U32.v len1) sub_rel1
+                                                (U32.v i2) (U32.v i2 + U32.v len2) sub_rel2
 
 
 /// A buffer ``b`` is equal to its "largest" sub-buffer, at index 0 and
 /// length ``len b``.
 
-abstract val gsub_zero_length (#a:Type0) (#rrel:srel a) (#rel:srel a) (b:mbuffer a rrel rel)
-  :Lemma (compatible_sub b 0ul (len b) rel /\ b == gsub b 0ul (len b) rel)
-let gsub_zero_length #_ #_ #rel b = lemma_sub_compatilibity_is_reflexive (length b) rel
+let gsub_zero_length #_ #_ #rel b = Seq.lemma_seq_sub_compatilibity_is_reflexive (length b) rel
 
-
-/// The contents of a sub-buffer is the corresponding slice of the
-/// contents of its enclosing buffer.
-
-abstract val as_seq_gsub (#a:Type0) (#rrel:srel a) (#rel:srel a)
-  (h:HS.mem) (b:mbuffer a rrel rel) (i:U32.t) (len:U32.t) (sub_rel:srel a)
-  :Lemma (requires (U32.v i + U32.v len <= length b /\ compatible_sub b i len sub_rel))
-         (ensures (as_seq h (gsub b i len sub_rel) == Seq.slice (as_seq h b) (U32.v i) (U32.v i + U32.v len)))
-         [SMTPat (as_seq h (gsub b i len sub_rel))]
 let as_seq_gsub #_ #_ #_ h b i len _ =
   match b with
   | Null -> ()
@@ -608,7 +256,7 @@ let unused_in_ubuffer_preserved (#a:Type0) (#rrel:srel a) (#rel:srel a)
   : Lemma (requires (b `unused_in` h))
           (ensures (ubuffer_preserved #(frameOf b) #(as_addr b) (ubuffer_of_buffer b) h h'))
   = Classical.move_requires (fun b -> live_not_unused_in h b) b;
-    live_null a #rrel #rel h;
+    live_null a rrel rel h;
     null_unique b;
     unused_in_equiv b h;
     addr_unused_in_ubuffer_preserved #(frameOf b) #(as_addr b) (ubuffer_of_buffer b) h h'
@@ -619,6 +267,7 @@ let ubuffer_includes' (larger smaller: ubuffer_) : GTot Type0 =
   larger.b_offset <= smaller.b_offset /\
   smaller.b_offset + smaller.b_length <= larger.b_offset + larger.b_length
 
+(* TODO: added this because of #606, now that it is fixed, we may not need it anymore *)
 let ubuffer_includes0 (#r1 #r2:HS.rid) (#a1 #a2:nat) (larger:ubuffer r1 a1) (smaller:ubuffer r2 a2) =
   r1 == r2 /\ a1 == a2 /\ ubuffer_includes' (G.reveal larger) (G.reveal smaller)
 
@@ -626,7 +275,6 @@ val ubuffer_includes (#r: HS.rid) (#a: nat) (larger smaller: ubuffer r a) : GTot
 
 let ubuffer_includes #r #a larger smaller = ubuffer_includes0 larger smaller
   
-
 val ubuffer_includes_refl (#r: HS.rid) (#a: nat) (b: ubuffer r a) : Lemma
   (b `ubuffer_includes` b)
 
@@ -665,6 +313,7 @@ let ubuffer_disjoint' (x1 x2: ubuffer_) : GTot Type0 =
     (x1.b_offset + x1.b_length <= x2.b_offset \/
      x2.b_offset + x2.b_length <= x1.b_offset))
 
+(* TODO: added this because of #606, now that it is fixed, we may not need it anymore *)
 let ubuffer_disjoint0 (#r1 #r2:HS.rid) (#a1 #a2:nat) (b1:ubuffer r1 a1) (b2:ubuffer r2 a2) =
   r1 == r2 /\ a1 == a2 /\
   ubuffer_disjoint' (G.reveal b1) (G.reveal b2)
@@ -878,236 +527,63 @@ let cls : MG.cls ubuffer = MG.Cls #ubuffer
   (fun #r #a x h1 h2 h3 -> ubuffer_preserved_trans x h1 h2 h3)
   (fun #r #a b h1 h2 f -> same_mreference_ubuffer_preserved b h1 h2 f)
 
-/// # The modifies clause
-///
-/// The modifies clause for regions, references and buffers.
-/// ==========================================================
-///
-/// This module presents the modifies clause, a way to track the set
-/// of memory locations modified by a stateful Low* (or even F*)
-/// program. The basic principle of modifies clauses is that any
-/// location that is disjoint from a set of memory locations modified
-/// by an operation is preserved by that operation.
-///
-/// We start by specifying a monoid of sets of memory locations. From
-/// a rough high-level view, ``loc`` is the type of sets of memory
-/// locations, equipped with an identity element ``loc_none``,
-/// representing the empty set, and an associative and commutative
-/// operator, ``loc_union``, representing the union of two sets of
-/// memory locations.
-///
-/// Moreover, ``loc_union`` is idempotent, which is useful to cut SMT
-/// matching loops with ``modifies_trans`` and ``modifies_refl`` below.
-
-abstract val loc :Type0
 let loc = MG.loc cls
 
-abstract val loc_none :loc
 let loc_none = MG.loc_none
 
-abstract val loc_union (s1 s2: loc) :GTot loc
 let loc_union = MG.loc_union
 
-abstract val loc_union_idem (s:loc) :Lemma (loc_union s s == s)
-                                           [SMTPat (loc_union s s)]
 let loc_union_idem = MG.loc_union_idem
 
-abstract val loc_union_comm (s1 s2:loc) :Lemma (loc_union s1 s2 == loc_union s2 s1)
-                                               [SMTPat (loc_union s1 s2)]
 let loc_union_comm = MG.loc_union_comm
 
-abstract val loc_union_assoc (s1 s2 s3:loc) :Lemma (loc_union s1 (loc_union s2 s3) == loc_union (loc_union s1 s2) s3)
 let loc_union_assoc = MG.loc_union_assoc
 
-let loc_union_idem_1 (s1 s2:loc)
-  :Lemma (loc_union s1 (loc_union s1 s2) == loc_union s1 s2)
-         [SMTPat (loc_union s1 (loc_union s1 s2) == loc_union s1 s2)]
-  = loc_union_assoc s1 s1 s2
-
-let loc_union_idem_2 (s1 s2:loc)
-  :Lemma (loc_union (loc_union s1 s2) s2 == loc_union s1 s2)
-         [SMTPat (loc_union (loc_union s1 s2) s2)]
-  = loc_union_assoc s1 s2 s2
-
-abstract val loc_union_loc_none_l (s:loc) :Lemma (loc_union loc_none s == s)
-                                                 [SMTPat (loc_union loc_none s)]
 let loc_union_loc_none_l = MG.loc_union_loc_none_l
 
-abstract val loc_union_loc_none_r (s:loc) :Lemma (loc_union s loc_none == s)
-                                                 [SMTPat (loc_union s loc_none)]
 let loc_union_loc_none_r = MG.loc_union_loc_none_r
 
-
-/// ``loc_buffer b`` is the set of memory locations associated to a buffer ``b``.
-
-abstract val loc_buffer (#a:Type0) (#rrel:srel a) (#rel:srel a) (b:mbuffer a rrel rel) :GTot loc
 let loc_buffer #_ #_ #_ b =
   if g_is_null b then MG.loc_none
   else MG.loc_of_aloc #_ #_ #(frameOf b) #(as_addr b) (ubuffer_of_buffer b)
 
-abstract val loc_buffer_null (a:Type0) (rrel:srel a) (rel:srel a)  (* TODO: candidate for wrapper *)
-  :Lemma (loc_buffer (null #a #rrel #rel) == loc_none)
-         [SMTPat (loc_buffer (null #a #rrel #rel))]
 let loc_buffer_null _ _ _ = ()
 
-
-/// ``loc_addresses r n`` is the set of memory locations associated to a
-/// set of addresses ``n`` in a given region ``r``.
-
-abstract val loc_addresses (preserve_liveness:bool) (r:HS.rid) (n:Set.set nat) :GTot loc
 let loc_addresses = MG.loc_addresses
 
-unfold let loc_addr_of_buffer (#a:Type0) (#rrel:srel a) (#rel:srel a) (b:mbuffer a rrel rel) :GTot loc =
-  loc_addresses false (frameOf b) (Set.singleton (as_addr b))
-
-
-/// ``loc_regions r`` is the set of memory locations associated to a set
-/// ``r`` of regions.
-
-abstract val loc_regions (preserve_liveness:bool) (r:Set.set HS.rid) :GTot loc
 let loc_regions = MG.loc_regions
 
-
-/// ``loc_mreference b`` is the set of memory locations associated to a
-/// reference ``b``, which is actually the set of memory locations
-/// associated to the address of ``b``.
-
-unfold let loc_mreference (#a:Type0) (#p:Preorder.preorder a) (b:HS.mreference a p) :GTot loc
-  = loc_addresses true (HS.frameOf b) (Set.singleton (HS.as_addr b))
-
-unfold
-let loc_freed_mreference (#a:Type0) (#p:Preorder.preorder a) (b:HS.mreference a p) :GTot loc
-  = loc_addresses false (HS.frameOf b) (Set.singleton (HS.as_addr b))
-
-
-/// ``loc_region_only r`` is the set of memory locations associated to a
-/// region ``r`` but not any region ``r'`` that extends ``r`` (in the sense
-/// of ``FStar.HyperStack.extends``.)
-
-unfold
-let loc_region_only (preserve_liveness:bool) (r:HS.rid) :GTot loc
-  = loc_regions preserve_liveness (Set.singleton r)
-
-
-/// ``loc_all_regions_from r`` is the set of all memory locations
-/// associated to a region ``r`` and any region ``r'`` that transitively
-/// extends ``r`` (in the sense of ``FStar.HyperStack.extends``,
-/// e.g. nested stack frames.)
-
-unfold
-let loc_all_regions_from (preserve_liveness:bool) (r:HS.rid) :GTot loc
-  = loc_regions preserve_liveness (HS.mod_set (Set.singleton r))
-
-
-/// We equip the ``loc`` monoid of sets of memory locations with an
-/// inclusion relation, ``loc_includes``, which is a preorder compatible
-/// with ``loc_union``. Although we consider sets of memory locations,
-/// we do not specify them using any F* set library such as
-/// ``FStar.Set``, ``FStar.TSet`` or ``FStar.GSet``, because ``loc_includes``
-/// encompasses more than just set-theoretic inclusion.
-
-abstract val loc_includes (s1 s2:loc) :GTot Type0
 let loc_includes = MG.loc_includes
 
-abstract val loc_includes_refl (s:loc)
-  :Lemma (loc_includes s s)
-         [SMTPat (loc_includes s s)]
 let loc_includes_refl = MG.loc_includes_refl
 
-abstract val loc_includes_trans (s1 s2 s3:loc)
-  :Lemma (requires (loc_includes s1 s2 /\ loc_includes s2 s3))
-         (ensures (loc_includes s1 s3))
 let loc_includes_trans = MG.loc_includes_trans
 
-let loc_includes_trans_backwards (s1 s2 s3:loc)
-  :Lemma (requires (loc_includes s1 s2 /\ loc_includes s2 s3))
-         (ensures  (loc_includes s1 s3))
-  [SMTPat (loc_includes s1 s3); SMTPat (loc_includes s2 s3)]
-  = loc_includes_trans s1 s2 s3
-
-abstract val loc_includes_union_r (s s1 s2:loc)
-  :Lemma (requires (loc_includes s s1 /\ loc_includes s s2))
-         (ensures (loc_includes s (loc_union s1 s2)))
 let loc_includes_union_r = MG.loc_includes_union_r
 
-abstract val loc_includes_union_l (s1 s2 s:loc)
-  :Lemma (requires (loc_includes s1 s \/ loc_includes s2 s))
-         (ensures (loc_includes (loc_union s1 s2) s))
 let loc_includes_union_l = MG.loc_includes_union_l
 
-let loc_includes_union_r' (s s1 s2:loc)
-  :Lemma (loc_includes s (loc_union s1 s2) <==> (loc_includes s s1 /\ loc_includes s s2))
-         [SMTPat (loc_includes s (loc_union s1 s2))]
-  = Classical.move_requires (loc_includes_union_r s s1) s2;
-    Classical.move_requires (loc_includes_union_l s1 s2) s1;
-    Classical.move_requires (loc_includes_union_l s1 s2) s2;
-    Classical.move_requires (loc_includes_trans s (loc_union s1 s2)) s1;
-    Classical.move_requires (loc_includes_trans s (loc_union s1 s2)) s2
-
-abstract val loc_includes_none (s:loc)
-  :Lemma (loc_includes s loc_none)
-         [SMTPat (loc_includes s loc_none)]
 let loc_includes_none = MG.loc_includes_none
 
-private abstract val loc_includes_buffer (#a:Type0) (#rrel1:srel a) (#rrel2:srel a) (#rel1:srel a) (#rel2:srel a)
+val loc_includes_buffer (#a:Type0) (#rrel1:srel a) (#rrel2:srel a) (#rel1:srel a) (#rel2:srel a)
   (b1:mbuffer a rrel1 rel1) (b2:mbuffer a rrel2 rel2)
   :Lemma (requires (frameOf b1 == frameOf b2 /\ as_addr b1 == as_addr b2 /\
                     ubuffer_includes0 #(frameOf b1) #(frameOf b2) #(as_addr b1) #(as_addr b2) (ubuffer_of_buffer b1) (ubuffer_of_buffer b2)))
          (ensures  (loc_includes (loc_buffer b1) (loc_buffer b2)))
-
 let loc_includes_buffer #t #_ #_ #_ #_ b1 b2 =
   let t1 = ubuffer (frameOf b1) (as_addr b1) in
   MG.loc_includes_aloc #_ #cls #(frameOf b1) #(as_addr b1) (ubuffer_of_buffer b1) (ubuffer_of_buffer b2 <: t1)
 
-/// If a buffer ``b1`` includes a buffer ``b2`` in the sense of the buffer
-/// theory (see ``LowStar.Buffer.includes``), then so are their
-/// corresponding sets of memory locations.
-
-abstract val loc_includes_gsub_buffer_r
-  (l:loc)
-  (#a:Type0) (#rrel:srel a) (#rel:srel a)
-  (b:mbuffer a rrel rel) (i:UInt32.t) (len:UInt32.t) (sub_rel:srel a)
-: Lemma (requires (UInt32.v i + UInt32.v len <= (length b) /\
-                   compatible_sub b i len sub_rel /\
-                   loc_includes l (loc_buffer b)))
-        (ensures  (loc_includes l (loc_buffer (gsub b i len sub_rel))))
-        [SMTPat (loc_includes l (loc_buffer (gsub b i len sub_rel)))]
 let loc_includes_gsub_buffer_r l #_ #_ #_ b i len sub_rel =
   let b' = gsub b i len sub_rel in
   loc_includes_buffer b b';
   loc_includes_trans l (loc_buffer b) (loc_buffer b')
 
-let loc_includes_gsub_buffer_r' (#a:Type0) (#rrel:srel a) (#rel:srel a)
-  (b:mbuffer a rrel rel) (i:UInt32.t) (len:UInt32.t) (sub_rel:srel a)
-  :Lemma (requires (UInt32.v i + UInt32.v len <= (length b) /\ compatible_sub b i len sub_rel))
-         (ensures  (loc_includes (loc_buffer b) (loc_buffer (gsub b i len sub_rel))))
-         [SMTPat (gsub b i len sub_rel)]
-  = ()
-
-val loc_includes_gsub_buffer_l (#a:Type0) (#rrel #rel:srel a) (b:mbuffer a rrel rel)
-  (i1:UInt32.t) (len1:UInt32.t) (sub_rel1:srel a)
-  (i2:UInt32.t) (len2:UInt32.t) (sub_rel2:srel a)
-  :Lemma (requires (UInt32.v i1 + UInt32.v len1 <= (length b) /\
-                    UInt32.v i1 <= UInt32.v i2 /\ UInt32.v i2 + UInt32.v len2 <= UInt32.v i1 + UInt32.v len1 /\
-		    compatible_sub b i1 len1 sub_rel1 /\ compatible_sub b i2 len2 sub_rel2))
-         (ensures  (loc_includes (loc_buffer (gsub b i1 len1 sub_rel1)) (loc_buffer (gsub b i2 len2 sub_rel2))))
-         [SMTPat (gsub b i1 len1 sub_rel1); SMTPat (gsub b i2 len2 sub_rel2)]
 let loc_includes_gsub_buffer_l #_ #_ #rel b i1 len1 sub_rel1 i2 len2 sub_rel2 =
   let b1 = gsub b i1 len1 sub_rel1 in
   let b2 = gsub b i2 len2 sub_rel2 in
-  //lemma_sub_compatibility_is_transitive1 (length b) rel (U32.v i1) (U32.v len1) sub_rel1 (U32.v i2) (U32.v len2) sub_rel2;
-  //let b2 = gsub b1 (U32.sub i2 i1) len2 sub_rel2 in
   loc_includes_buffer b1 b2
 
-/// If the contents of a buffer are equal in two given heaps, then so
-/// are the contents of any of its sub-buffers.
-
-val loc_includes_as_seq (#a:Type0) (#rrel1 #rrel2 #rel1 #rel2:srel a)
-  (h1 h2:HS.mem) (larger:mbuffer a rrel1 rel1) (smaller:mbuffer a rrel2 rel2)
-  :Lemma (requires (loc_includes (loc_buffer larger) (loc_buffer smaller) /\
-                    as_seq h1 larger == as_seq h2 larger /\
-		    (live h1 larger \/ live h1 smaller) /\ (live h2 larger \/ live h2 smaller)))
-         (ensures  (as_seq h1 smaller == as_seq h2 smaller))
 #push-options "--z3rlimit 20"
 let loc_includes_as_seq #_ #rrel1 #rrel2 #_ #_ h1 h2 larger smaller =
   if Null? smaller then () else
@@ -1124,260 +600,29 @@ let loc_includes_as_seq #_ #rrel1 #rrel2 #_ #_ h1 h2 larger smaller =
   end
 #pop-options
 
-
-/// Given a buffer ``b``, if its address is in a set ``s`` of addresses in
-/// the region of ``b``, then the set of memory locations corresponding
-/// to ``b`` is included in the set of memory locations corresponding to
-/// the addresses in ``s`` in region ``r``.
-///
-/// In particular, the set of memory locations corresponding to a
-/// buffer is included in the set of memory locations corresponding to
-/// its region and address.
-
-val loc_includes_addresses_buffer (#a:Type0) (#rrel #rel:srel a)
-  (preserve_liveness:bool) (r:HS.rid) (s:Set.set nat) (p:mbuffer a rrel rel)
-  :Lemma (requires (frameOf p == r /\ Set.mem (as_addr p) s))
-         (ensures  (loc_includes (loc_addresses preserve_liveness r s) (loc_buffer p)))
-         [SMTPat (loc_includes (loc_addresses preserve_liveness r s) (loc_buffer p))]
 let loc_includes_addresses_buffer #_ #_ #_ preserve_liveness r s p =
   MG.loc_includes_addresses_aloc #_ #cls preserve_liveness r s #(as_addr p) (ubuffer_of_buffer p)
 
-let loc_includes_addresses_buffer' (#a:Type0) (#rrel #rel:srel a) (b:mbuffer a rrel rel)
-  :Lemma (loc_includes (loc_addresses true (frameOf b) (Set.singleton (as_addr b))) (loc_buffer b))
-         [SMTPat (loc_buffer b)]
-  = ()
-
-/// The set of memory locations corresponding to a buffer is included
-/// in the set of memory locations corresponding to its region.
-
-val loc_includes_region_buffer (#a:Type0) (#rrel #rel:srel a)
-  (preserve_liveness:bool) (s:Set.set HS.rid) (b:mbuffer a rrel rel)
-  :Lemma (requires (Set.mem (frameOf b) s))
-         (ensures (loc_includes (loc_regions preserve_liveness s) (loc_buffer b)))
-         [SMTPat (loc_includes (loc_regions preserve_liveness s) (loc_buffer b))]
 let loc_includes_region_buffer #_ #_ #_ preserve_liveness s b =
   MG.loc_includes_region_aloc #_ #cls preserve_liveness s #(frameOf b) #(as_addr b) (ubuffer_of_buffer b)
 
-let loc_includes_region_buffer' (#a:Type0) (#rrel #rel:srel a) (b:mbuffer a rrel rel)
-  :Lemma (loc_includes (loc_regions true (Set.singleton (frameOf b))) (loc_buffer b))
-         [SMTPat (loc_buffer b)]
-  = ()
-
-
-/// If a region ``r`` is in a set of regions ``s``, then the set of memory
-/// locations corresponding to a set of addresses ``a`` in ``r`` is
-/// included in the set of memory locations corresponding to the
-/// regions in ``s``.
-///
-/// In particular, the the set of memory locations corresponding to a
-/// set of addresses ``a`` in a given region ``r`` is included in the set
-/// of memory locations corresponding to region ``r``.
-
-val loc_includes_region_addresses
-  (preserve_liveness1: bool)
-  (preserve_liveness2: bool)
-  (s: Set.set HS.rid)
-  (r: HS.rid)
-  (a: Set.set nat)
-: Lemma
-  (requires (Set.mem r s))
-  (ensures (loc_includes (loc_regions preserve_liveness1 s) (loc_addresses preserve_liveness2 r a)))
-  [SMTPat (loc_includes (loc_regions preserve_liveness1 s) (loc_addresses preserve_liveness2 r a))]
 let loc_includes_region_addresses = MG.loc_includes_region_addresses #_ #cls
 
-let loc_includes_region_addresses'
-  (preserve_liveness: bool)
-  (r: HS.rid)
-  (a: Set.set nat)
-: Lemma
-  (loc_includes (loc_regions true (Set.singleton r)) (loc_addresses preserve_liveness r a))
-  [SMTPat (loc_addresses preserve_liveness r a)]
-= ()
-
-/// If a set of region identifiers ``s1`` includes a set of region
-/// identifiers ``s2``, then so are their corresponding sets of memory
-/// locations.
-
-val loc_includes_region_region
-  (preserve_liveness1: bool)
-  (preserve_liveness2: bool)
-  (s1 s2: Set.set HS.rid)
-: Lemma
-  (requires ((preserve_liveness1 ==> preserve_liveness2) /\ Set.subset s2 s1))
-  (ensures (loc_includes (loc_regions preserve_liveness1 s1) (loc_regions preserve_liveness2 s2)))
-  [SMTPat (loc_includes (loc_regions preserve_liveness1 s1) (loc_regions preserve_liveness2 s2))]
 let loc_includes_region_region = MG.loc_includes_region_region #_ #cls
 
-let loc_includes_region_region'
-  (preserve_liveness: bool)
-  (s: Set.set HS.rid)
-: Lemma
-  (loc_includes (loc_regions false s) (loc_regions preserve_liveness s))
-  [SMTPat (loc_regions preserve_liveness s)]
-= ()
-
-/// The following lemma can act as a cut when reasoning with sets of
-/// memory locations corresponding to sets of regions.
-
-val loc_includes_region_union_l
-  (preserve_liveness: bool)
-  (l: loc)
-  (s1 s2: Set.set HS.rid)
-: Lemma
-  (requires (loc_includes l (loc_regions preserve_liveness (Set.intersect s2 (Set.complement s1)))))
-  (ensures (loc_includes (loc_union (loc_regions preserve_liveness s1) l) (loc_regions preserve_liveness s2)))
-  [SMTPat (loc_includes (loc_union (loc_regions preserve_liveness s1) l) (loc_regions preserve_liveness s2))]
 let loc_includes_region_union_l = MG.loc_includes_region_union_l
 
-
-/// If a set of addresses ``s1`` includes a set of addresses ``s2``,
-/// then so are their corresponding memory locations
-val loc_includes_addresses_addresses
-  (preserve_liveness1 preserve_liveness2: bool)
-  (r: HS.rid)
-  (s1 s2: Set.set nat)
-: Lemma
-  (requires ((preserve_liveness1 ==> preserve_liveness2) /\ Set.subset s2 s1))
-  (ensures (loc_includes (loc_addresses preserve_liveness1 r s1) (loc_addresses preserve_liveness2 r s2)))
 let loc_includes_addresses_addresses = MG.loc_includes_addresses_addresses cls
 
-let loc_includes_addresses_addresses_1
-  (preserve_liveness1 preserve_liveness2: bool)
-  (r1 r2: HS.rid)
-  (s1 s2: Set.set nat)
-: Lemma
-  (requires (r1 == r2 /\ (preserve_liveness1 ==> preserve_liveness2) /\ Set.subset s2 s1))
-  (ensures (loc_includes (loc_addresses preserve_liveness1 r1 s1) (loc_addresses preserve_liveness2 r2 s2)))
-  [SMTPat (loc_includes (loc_addresses preserve_liveness1 r1 s1) (loc_addresses preserve_liveness2 r2 s2))]
-= loc_includes_addresses_addresses preserve_liveness1 preserve_liveness2 r1 s1 s2
-
-let loc_includes_addresses_addresses_2
-  (preserve_liveness: bool)
-  (r: HS.rid)
-  (s: Set.set nat)
-: Lemma
-  (loc_includes (loc_addresses false r s) (loc_addresses preserve_liveness r s))
-  [SMTPat (loc_addresses preserve_liveness r s)]
-= ()
-
-/// Patterns with loc_includes, union on the left
-
-let loc_includes_union_l_buffer
-  (s1 s2:loc)
-  (#a:Type0) (#rrel #rel:srel a)
-  (b:mbuffer a rrel rel)
-  :Lemma (requires (loc_includes s1 (loc_buffer b) \/ loc_includes s2 (loc_buffer b)))
-         (ensures (loc_includes (loc_union s1 s2) (loc_buffer b)))
-         [SMTPat (loc_includes (loc_union s1 s2) (loc_buffer b))]
-  = loc_includes_union_l s1 s2 (loc_buffer b)
-
-let loc_includes_union_l_addresses
-  (s1 s2: loc)
-  (prf: bool)
-  (r: HS.rid)
-  (a: Set.set nat)
-: Lemma
-  (requires (loc_includes s1 (loc_addresses prf r a) \/ loc_includes s2 (loc_addresses prf r a)))
-  (ensures (loc_includes (loc_union s1 s2) (loc_addresses prf r a)))
-  [SMTPat (loc_includes (loc_union s1 s2) (loc_addresses prf r a))]
-= loc_includes_union_l s1 s2 (loc_addresses prf r a)
-
-let loc_includes_union_l_regions
-  (s1 s2: loc)
-  (prf: bool)
-  (r: Set.set HS.rid)
-: Lemma
-  (requires (loc_includes s1 (loc_regions prf r) \/ loc_includes s2 (loc_regions prf r)))
-  (ensures (loc_includes (loc_union s1 s2) (loc_regions prf r)))
-  [SMTPat (loc_includes (loc_union s1 s2) (loc_regions prf r))]
-= loc_includes_union_l s1 s2 (loc_regions prf r)
-
-/// Since inclusion encompasses more than just set-theoretic
-/// inclusion, we also need to specify disjointness accordingly, as a
-/// symmetric relation compatible with union.
-
-val loc_disjoint
-  (s1 s2: loc)
-: GTot Type0
 let loc_disjoint = MG.loc_disjoint
 
-[@"opaque_to_smt"]
-private let rec loc_disjoint_from_list (l:loc) (ls:list loc) :Type0 =
-  match ls with
-  | []    -> True
-  | hd::tl -> loc_disjoint l hd /\ loc_disjoint_from_list l tl
-
-[@"opaque_to_smt"]
-private let rec loc_pairwise_disjoint_aux (l:list loc) :Type0 =
-  match l with
-  | []    -> True
-  | hd::tl -> loc_disjoint_from_list hd tl /\ loc_pairwise_disjoint_aux tl
-
-(*
- * Use this to state pairwise disjointness for the locations in l
- * It is unfolded to conjunction of loc_disjoint for all pairs of locations in l
- *)
-[@"opaque_to_smt"]
-unfold let loc_pairwise_disjoint (l:list loc) :Type0 =
-  norm [iota; zeta; delta; delta_only ["LowStar.Buffer.loc_disjoint_from_list";
-                                       "LowStar.Buffer.loc_pairwise_disjoint_aux"]] (loc_pairwise_disjoint_aux l)
-
-val loc_disjoint_sym
-  (s1 s2: loc)
-: Lemma
-  (requires (loc_disjoint s1 s2))
-  (ensures (loc_disjoint s2 s1))
 let loc_disjoint_sym = MG.loc_disjoint_sym
 
-let loc_disjoint_sym'
-  (s1 s2: loc)
-: Lemma
-  (loc_disjoint s1 s2 <==> loc_disjoint s2 s1)
-  [SMTPat (loc_disjoint s1 s2)]
-= Classical.move_requires (loc_disjoint_sym s1) s2;
-  Classical.move_requires (loc_disjoint_sym s2) s1
-
-val loc_disjoint_none_r
-  (s: loc)
-: Lemma
-  (ensures (loc_disjoint s loc_none))
-  [SMTPat (loc_disjoint s loc_none)]
 let loc_disjoint_none_r = MG.loc_disjoint_none_r
 
-val loc_disjoint_union_r
-  (s s1 s2: loc)
-: Lemma
-  (requires (loc_disjoint s s1 /\ loc_disjoint s s2))
-  (ensures (loc_disjoint s (loc_union s1 s2)))
 let loc_disjoint_union_r = MG.loc_disjoint_union_r
 
-
-/// If two sets of memory locations are disjoint, then so are any two
-/// included sets of memory locations.
-
-val loc_disjoint_includes
-  (p1 p2 p1' p2' : loc)
-: Lemma
-  (requires (loc_includes p1 p1' /\ loc_includes p2 p2' /\ loc_disjoint p1 p2))
-  (ensures (loc_disjoint p1' p2'))
 let loc_disjoint_includes = MG.loc_disjoint_includes
-
-let loc_disjoint_union_r'
-  (s s1 s2: loc)
-: Lemma
-  (ensures (loc_disjoint s (loc_union s1 s2) <==> (loc_disjoint s s1 /\ loc_disjoint s s2)))
-  [SMTPat (loc_disjoint s (loc_union s1 s2))]
-= Classical.move_requires (loc_disjoint_union_r s s1) s2;
-  loc_includes_union_l s1 s2 s1;
-  loc_includes_union_l s1 s2 s2;
-  Classical.move_requires (loc_disjoint_includes s (loc_union s1 s2) s) s1;
-  Classical.move_requires (loc_disjoint_includes s (loc_union s1 s2) s) s2
-
-let loc_disjoint_includes_r (b1 : loc) (b2 b2': loc) : Lemma
-  (requires (loc_includes b2 b2' /\ loc_disjoint b1 b2))
-  (ensures (loc_disjoint b1 b2'))
-  [SMTPat (loc_disjoint b1 b2'); SMTPat (loc_includes b2 b2')]
-= loc_disjoint_includes b1 b2 b1 b2'
 
 val loc_disjoint_buffer (#a1 #a2:Type0) (#rrel1 #rel1:srel a1) (#rrel2 #rel2:srel a2)
   (b1:mbuffer a1 rrel1 rel1) (b2:mbuffer a2 rrel2 rel2)
@@ -1387,104 +632,19 @@ val loc_disjoint_buffer (#a1 #a2:Type0) (#rrel1 #rel1:srel a1) (#rrel2 #rel2:sre
 let loc_disjoint_buffer #_ #_ #_ #_ #_ #_ b1 b2 =
   MG.loc_disjoint_aloc_intro #_ #cls #(frameOf b1) #(as_addr b1) #(frameOf b2) #(as_addr b2) (ubuffer_of_buffer b1) (ubuffer_of_buffer b2)
 
-val loc_disjoint_gsub_buffer (#a:Type0) (#rrel:srel a) (#rel:srel a)
-  (b:mbuffer a rrel rel)
-  (i1:UInt32.t) (len1:UInt32.t) (sub_rel1:srel a)
-  (i2:UInt32.t) (len2:UInt32.t) (sub_rel2:srel a)
-  :Lemma (requires (UInt32.v i1 + UInt32.v len1 <= (length b) /\
-                    UInt32.v i2 + UInt32.v len2 <= (length b) /\
-		    compatible_sub b i1 len1 sub_rel1 /\ compatible_sub b i2 len2 sub_rel2 /\
-		    (UInt32.v i1 + UInt32.v len1 <= UInt32.v i2 \/
-                     UInt32.v i2 + UInt32.v len2 <= UInt32.v i1)))
-         (ensures  (loc_disjoint (loc_buffer (gsub b i1 len1 sub_rel1)) (loc_buffer (gsub b i2 len2 sub_rel2))))
-         [SMTPat (gsub b i1 len1 sub_rel1); SMTPat (gsub b i2 len2 sub_rel2)]
 let loc_disjoint_gsub_buffer #_ #_ #_ b i1 len1 sub_rel1 i2 len2 sub_rel2 =
   loc_disjoint_buffer (gsub b i1 len1 sub_rel1) (gsub b i2 len2 sub_rel2)
 
-
-/// If two sets of addresses correspond to different regions or are
-/// disjoint, then their corresponding sets of memory locations are
-/// disjoint.
-
-val loc_disjoint_addresses
-  (preserve_liveness1 preserve_liveness2: bool)
-  (r1 r2: HS.rid)
-  (n1 n2: Set.set nat)
-: Lemma
-  (requires (r1 <> r2 \/ Set.subset (Set.intersect n1 n2) Set.empty))
-  (ensures (loc_disjoint (loc_addresses preserve_liveness1 r1 n1) (loc_addresses preserve_liveness2 r2 n2)))
-  [SMTPat (loc_disjoint (loc_addresses preserve_liveness1 r1 n1) (loc_addresses preserve_liveness2 r2 n2))]
 let loc_disjoint_addresses = MG.loc_disjoint_addresses_intro #_ #cls
 
-
-/// If two sets of region identifiers are disjoint, then so are their
-/// corresponding sets of memory locations.
-
-val loc_disjoint_regions
-  (preserve_liveness1: bool)
-  (preserve_liveness2: bool)
-  (rs1 rs2: Set.set HS.rid)
-: Lemma
-  (requires (Set.subset (Set.intersect rs1 rs2) Set.empty))
-  (ensures (loc_disjoint (loc_regions preserve_liveness1 rs1) (loc_regions preserve_liveness2 rs2)))
-  [SMTPat (loc_disjoint (loc_regions preserve_liveness1 rs1) (loc_regions preserve_liveness2 rs2))]
 let loc_disjoint_regions = MG.loc_disjoint_regions #_ #cls
 
-/// The modifies clauses proper.
-///
-/// Let ``s`` be a set of memory locations, and ``h1`` and ``h2`` be two
-/// memory states. Then, ``s`` is modified from ``h1`` to ``h2`` only if,
-/// any memory location disjoint from ``s`` is preserved from ``h1`` into
-/// ``h2``. Elimination lemmas illustrating this principle follow.
-
-val modifies
-  (s: loc)
-  (h1 h2: HS.mem)
-: GTot Type0
 let modifies = MG.modifies
 
-
-/// If a region ``r`` is disjoint from a set ``s`` of memory locations
-/// which is modified, then its liveness is preserved.
-
-val modifies_live_region
-  (s: loc)
-  (h1 h2: HS.mem)
-  (r: HS.rid)
-: Lemma
-  (requires (modifies s h1 h2 /\ loc_disjoint s (loc_region_only false r) /\ HS.live_region h1 r))
-  (ensures (HS.live_region h2 r))
 let modifies_live_region = MG.modifies_live_region
 
-/// If a reference ``b`` is disjoint from a set ``p`` of memory locations
-/// which is modified, then its liveness and contents are preserved.
-
-val modifies_mreference_elim
-  (#t: Type)
-  (#pre: Preorder.preorder t)
-  (b: HS.mreference t pre)
-  (p: loc)
-  (h h': HS.mem)
-: Lemma
-  (requires (
-    loc_disjoint (loc_mreference b) p /\
-    HS.contains h b /\
-    modifies p h h'
-  ))
-  (ensures (
-    HS.contains h' b /\
-    HS.sel h b == HS.sel h' b
-  ))
 let modifies_mreference_elim = MG.modifies_mreference_elim
 
-/// If a buffer ``b`` is disjoint from a set ``p`` of
-/// memory locations which is modified, then its liveness and contents
-/// are preserved.
-
-val modifies_buffer_elim (#a:Type0) (#rrel #rel:srel a)
-  (b:mbuffer a rrel rel) (p:loc) (h h':HS.mem)
-  :Lemma (requires (loc_disjoint (loc_buffer b) p /\ live h b /\ modifies p h h'))
-         (ensures  (live h' b /\ (as_seq h b == as_seq h' b)))
 let modifies_buffer_elim #_ #_ #_ b p h h' =
   if g_is_null b
   then
@@ -1494,360 +654,74 @@ let modifies_buffer_elim #_ #_ #_ b p h h' =
     ubuffer_preserved_elim b h h'
   end
 
-/// If the memory state does not change, then any memory location is
-/// modified (and, in particular, the empty set, ``loc_none``.)
-
-val modifies_refl
-  (s: loc)
-  (h: HS.mem)
-: Lemma
-  (modifies s h h)
-  [SMTPat (modifies s h h)]
 let modifies_refl = MG.modifies_refl
 
-/// If a set ``s2`` of memory locations is modified, then so is any set
-/// ``s1`` that includes ``s2``. In other words, it is always possible to
-/// weaken a modifies clause by widening its set of memory locations.
-
-val modifies_loc_includes
-  (s1: loc)
-  (h h': HS.mem)
-  (s2: loc)
-: Lemma
-  (requires (modifies s2 h h' /\ loc_includes s1 s2))
-  (ensures (modifies s1 h h'))
-  [SMTPat (modifies s1 h h'); SMTPat (modifies s2 h h')]
 let modifies_loc_includes = MG.modifies_loc_includes
 
-/// Some memory locations are tagged as liveness-insensitive: the
-/// liveness preservation of a memory location only depends on its
-/// disjointness from the liveness-sensitive memory locations of a
-/// modifies clause.
-
-val address_liveness_insensitive_locs: loc
 let address_liveness_insensitive_locs = MG.address_liveness_insensitive_locs _
 
-val region_liveness_insensitive_locs: loc
 let region_liveness_insensitive_locs = MG.region_liveness_insensitive_locs _
 
-val address_liveness_insensitive_buffer (#a:Type0) (#rrel #rel:srel a) (b:mbuffer a rrel rel)
-  :Lemma (address_liveness_insensitive_locs `loc_includes` (loc_buffer b))
-         [SMTPat (address_liveness_insensitive_locs `loc_includes` (loc_buffer b))]
 let address_liveness_insensitive_buffer #_ #_ #_ b =
   MG.loc_includes_address_liveness_insensitive_locs_aloc #_ #cls #(frameOf b) #(as_addr b) (ubuffer_of_buffer b)
 
-val address_liveness_insensitive_addresses (r: HS.rid) (a: Set.set nat) : Lemma
-  (address_liveness_insensitive_locs `loc_includes` (loc_addresses true r a))
-  [SMTPat (address_liveness_insensitive_locs `loc_includes` (loc_addresses true r a))]
 let address_liveness_insensitive_addresses =
   MG.loc_includes_address_liveness_insensitive_locs_addresses cls
 
-val region_liveness_insensitive_buffer (#a:Type0) (#rrel #rel:srel a) (b:mbuffer a rrel rel)
-  :Lemma (region_liveness_insensitive_locs `loc_includes` (loc_buffer b))
-         [SMTPat (region_liveness_insensitive_locs `loc_includes` (loc_buffer b))]
 let region_liveness_insensitive_buffer #_ #_ #_ b =
   MG.loc_includes_region_liveness_insensitive_locs_loc_of_aloc #_ cls #(frameOf b) #(as_addr b) (ubuffer_of_buffer b)
 
-val region_liveness_insensitive_addresses (preserve_liveness: bool) (r: HS.rid) (a: Set.set nat) : Lemma
-  (region_liveness_insensitive_locs `loc_includes` (loc_addresses preserve_liveness r a))
-  [SMTPat (region_liveness_insensitive_locs `loc_includes` (loc_addresses preserve_liveness r a))]
 let region_liveness_insensitive_addresses =
   MG.loc_includes_region_liveness_insensitive_locs_loc_addresses cls
 
-val region_liveness_insensitive_regions (rs: Set.set HS.rid) : Lemma
-  (region_liveness_insensitive_locs `loc_includes` (loc_regions true rs))
-  [SMTPat (region_liveness_insensitive_locs `loc_includes` (loc_regions true rs))]
 let region_liveness_insensitive_regions =
   MG.loc_includes_region_liveness_insensitive_locs_loc_regions cls
 
-val region_liveness_insensitive_address_liveness_insensitive:
-  squash (region_liveness_insensitive_locs `loc_includes` address_liveness_insensitive_locs)
 let region_liveness_insensitive_address_liveness_insensitive =
   MG.loc_includes_region_liveness_insensitive_locs_address_liveness_insensitive_locs cls
 
-val modifies_liveness_insensitive_mreference
-  (l1 l2 : loc)
-  (h h' : HS.mem)
-  (#t: Type)
-  (#pre: Preorder.preorder t)
-  (x: HS.mreference t pre)
-: Lemma
-  (requires (modifies (loc_union l1 l2) h h' /\ loc_disjoint l1 (loc_mreference x) /\ address_liveness_insensitive_locs `loc_includes` l2 /\ h `HS.contains` x))
-  (ensures (h' `HS.contains` x))
-  (* TODO: pattern *)
 let modifies_liveness_insensitive_mreference = MG.modifies_preserves_liveness
 
-val modifies_liveness_insensitive_buffer
-  (l1 l2:loc)
-  (h h':HS.mem)
-  (#a:Type0) (#rrel #rel:srel a)
-  (x:mbuffer a rrel rel)
-  :Lemma (requires (modifies (loc_union l1 l2) h h' /\ loc_disjoint l1 (loc_buffer x) /\ address_liveness_insensitive_locs `loc_includes` l2 /\ live h x))
-         (ensures  (live h' x))
-  (* TODO: pattern *)
 let modifies_liveness_insensitive_buffer l1 l2 h h' #_ #_ #_ x =
-  if g_is_null x
-  then ()
+  if g_is_null x then ()
   else
     liveness_preservation_intro h h' x (fun t' pre r ->
-      MG.modifies_preserves_liveness_strong l1 l2 h h' r (ubuffer_of_buffer x)
-    )
+      MG.modifies_preserves_liveness_strong l1 l2 h h' r (ubuffer_of_buffer x))
 
-let modifies_liveness_insensitive_mreference_weak
-  (l : loc)
-  (h h' : HS.mem)
-  (#t: Type)
-  (#pre: Preorder.preorder t)
-  (x: HS.mreference t pre)
-: Lemma
-  (requires (modifies l h h' /\ address_liveness_insensitive_locs `loc_includes` l /\ h `HS.contains` x))
-  (ensures (h' `HS.contains` x))
-= modifies_liveness_insensitive_mreference loc_none l h h' x
-
-let modifies_liveness_insensitive_buffer_weak
-  (l:loc)
-  (h h':HS.mem)
-  (#a:Type0) (#rrel #rel:srel a)
-  (x:mbuffer a rrel rel)
-  :Lemma (requires (modifies l h h' /\ address_liveness_insensitive_locs `loc_includes` l /\ live h x))
-         (ensures  (live h' x))
-  = modifies_liveness_insensitive_buffer loc_none l h h' x
-
-val modifies_liveness_insensitive_region
-  (l1 l2 : loc)
-  (h h' : HS.mem)
-  (x: HS.rid)
-: Lemma
-  (requires (modifies (loc_union l1 l2) h h' /\ loc_disjoint l1 (loc_region_only false x) /\ region_liveness_insensitive_locs `loc_includes` l2 /\ HS.live_region h x))
-  (ensures (HS.live_region h' x))
-  (* TODO: pattern *)
 let modifies_liveness_insensitive_region = MG.modifies_preserves_region_liveness
 
-val modifies_liveness_insensitive_region_mreference
-  (l1 l2 : loc)
-  (h h' : HS.mem)
-  (#t: Type)
-  (#pre: Preorder.preorder t)
-  (x: HS.mreference t pre)
-: Lemma
-  (requires (modifies (loc_union l1 l2) h h' /\ loc_disjoint l1 (loc_mreference x) /\ region_liveness_insensitive_locs `loc_includes` l2 /\ HS.live_region h (HS.frameOf x)))
-  (ensures (HS.live_region h' (HS.frameOf x)))
-  (* TODO: pattern *)
 let modifies_liveness_insensitive_region_mreference = MG.modifies_preserves_region_liveness_reference
 
-val modifies_liveness_insensitive_region_buffer
-  (l1 l2:loc)
-  (h h':HS.mem)
-  (#a:Type0) (#rrel #rel:srel a)
-  (x:mbuffer a rrel rel)
-  :Lemma (requires (modifies (loc_union l1 l2) h h' /\ loc_disjoint l1 (loc_buffer x) /\ region_liveness_insensitive_locs `loc_includes` l2 /\ HS.live_region h (frameOf x)))
-         (ensures  (HS.live_region h' (frameOf x)))
-  (* TODO: pattern *)
 let modifies_liveness_insensitive_region_buffer l1 l2 h h' #_ #_ #_ x =
-  if g_is_null x
-  then ()
-  else
-    MG.modifies_preserves_region_liveness_aloc l1 l2 h h' #(frameOf x) #(as_addr x) (ubuffer_of_buffer x)
+  if g_is_null x then ()
+  else MG.modifies_preserves_region_liveness_aloc l1 l2 h h' #(frameOf x) #(as_addr x) (ubuffer_of_buffer x)
 
-let modifies_liveness_insensitive_region_weak
-  (l2 : loc)
-  (h h' : HS.mem)
-  (x: HS.rid)
-: Lemma
-  (requires (modifies l2 h h' /\ region_liveness_insensitive_locs `loc_includes` l2 /\ HS.live_region h x))
-  (ensures (HS.live_region h' x))
-= modifies_liveness_insensitive_region loc_none l2 h h' x
-
-let modifies_liveness_insensitive_region_mreference_weak
-  (l2 : loc)
-  (h h' : HS.mem)
-  (#t: Type)
-  (#pre: Preorder.preorder t)
-  (x: HS.mreference t pre)
-: Lemma
-  (requires (modifies l2 h h' /\ region_liveness_insensitive_locs `loc_includes` l2 /\ HS.live_region h (HS.frameOf x)))
-  (ensures (HS.live_region h' (HS.frameOf x)))
-= modifies_liveness_insensitive_region_mreference loc_none l2 h h' x
-
-let modifies_liveness_insensitive_region_buffer_weak
-  (l2:loc)
-  (h h':HS.mem)
-  (#a:Type0) (#rrel #rel:srel a)
-  (x:mbuffer a rrel rel)
-  :Lemma (requires (modifies l2 h h' /\ region_liveness_insensitive_locs `loc_includes` l2 /\ HS.live_region h (frameOf x)))
-         (ensures  (HS.live_region h' (frameOf x)))
-  = modifies_liveness_insensitive_region_buffer loc_none l2 h h' x
-
-
-/// Modifies clauses are transitive. This lemma is the most general
-/// one.
-
-val modifies_trans
-  (s12: loc)
-  (h1 h2: HS.mem)
-  (s23: loc)
-  (h3: HS.mem)
-: Lemma
-  (requires (modifies s12 h1 h2 /\ modifies s23 h2 h3))
-  (ensures (modifies (loc_union s12 s23) h1 h3))
-  [SMTPat (modifies s12 h1 h2); SMTPat (modifies s23 h2 h3)]
 let modifies_trans = MG.modifies_trans
 
-/// Regions that are not live can be removed from sets of memory
-/// locations that are modified.
-
-val modifies_only_live_regions
-  (rs: Set.set HS.rid)
-  (l: loc)
-  (h h' : HS.mem)
-: Lemma
-  (requires (
-    modifies (loc_union (loc_regions false rs) l) h h' /\
-    (forall r . Set.mem r rs ==> (~ (HS.live_region h r)))
-  ))
-  (ensures (modifies l h h'))
 let modifies_only_live_regions = MG.modifies_only_live_regions
 
-/// As a consequence, fresh regions can be removed from modifies
-/// clauses.
-
-val no_upd_fresh_region: r:HS.rid -> l:loc -> h0:HS.mem -> h1:HS.mem -> Lemma
-  (requires (HS.fresh_region r h0 h1 /\ modifies (loc_union (loc_all_regions_from false r) l) h0 h1))
-  (ensures  (modifies l h0 h1))
-  [SMTPat (HS.fresh_region r h0 h1); SMTPat (modifies l h0 h1)]
 let no_upd_fresh_region = MG.no_upd_fresh_region
 
-val fresh_frame_modifies (h0 h1: HS.mem) : Lemma
-  (requires (HS.fresh_frame h0 h1))
-  (ensures (modifies loc_none h0 h1))
 let fresh_frame_modifies = MG.fresh_frame_modifies #_ cls
 
-val new_region_modifies (m0: HS.mem) (r0: HS.rid) (col: option int) : Lemma
-  (requires (HST.is_eternal_region r0 /\ HS.live_region m0 r0 /\ (None? col \/ HS.is_eternal_color (Some?.v col))))
-  (ensures (
-    let (_, m1) = HS.new_eternal_region m0 r0 col in
-    modifies loc_none m0 m1
-  ))
-  [SMTPat (HS.new_eternal_region m0 r0 col)]
 let new_region_modifies = MG.new_region_modifies #_ cls
 
-val popped_modifies (h0 h1: HS.mem) : Lemma
-  (requires (HS.popped h0 h1))
-  (ensures (modifies (loc_region_only false (HS.get_tip h0)) h0 h1))
 let popped_modifies = MG.popped_modifies #_ cls
 
-/// Stack discipline: any stack frame (and all its transitively
-/// extending regions) that is pushed, modified and popped can be
-/// removed from a modifies clause.
-
-val modifies_fresh_frame_popped
-  (h0 h1: HS.mem)
-  (s: loc)
-  (h2 h3: HS.mem)
-: Lemma
-  (requires (
-    HS.fresh_frame h0 h1 /\
-    modifies (loc_union (loc_all_regions_from false (HS.get_tip h1)) s) h1 h2 /\
-    (HS.get_tip h2) == (HS.get_tip h1) /\
-    HS.popped h2 h3
-  ))
-  (ensures (
-    modifies s h0 h3 /\
-    (HS.get_tip h3) == HS.get_tip h0
-  ))
-  [SMTPat (HS.fresh_frame h0 h1); SMTPat (HS.popped h2 h3); SMTPat (modifies s h0 h3)]
 let modifies_fresh_frame_popped = MG.modifies_fresh_frame_popped
 
-
-/// Compatibility lemmas to rescue modifies clauses specified in the
-/// standard F* HyperStack library.
-
-val modifies_loc_regions_intro
-  (rs: Set.set HS.rid)
-  (h1 h2: HS.mem)
-: Lemma
-  (requires (HS.modifies rs h1 h2))
-  (ensures (modifies (loc_regions true rs) h1 h2))
 let modifies_loc_regions_intro = MG.modifies_loc_regions_intro #_ #cls
 
-val modifies_loc_addresses_intro
-  (r: HS.rid)
-  (a: Set.set nat)
-  (l: loc)
-  (h1 h2: HS.mem)
-: Lemma
-  (requires (
-    HS.live_region h2 r /\
-    modifies (loc_union (loc_region_only false r) l) h1 h2 /\
-    HS.modifies_ref r a h1 h2
-  ))
-  (ensures (modifies (loc_union (loc_addresses true r a) l) h1 h2))
 let modifies_loc_addresses_intro = MG.modifies_loc_addresses_intro #_ #cls
 
-/// Modifies clauses for allocating a reference: nothing is
-/// modified. (In particular, a modifies clause does not track
-/// memory locations that are created.)
-
-val modifies_ralloc_post
-  (#a: Type)
-  (#rel: Preorder.preorder a)
-  (i: HS.rid)
-  (init: a)
-  (h: HS.mem)
-  (x: HST.mreference a rel { HST.is_eternal_region (HS.frameOf x) } )
-  (h' : HS.mem)
-: Lemma
-  (requires (HST.ralloc_post i init h x h'))
-  (ensures (modifies loc_none h h'))
-  [SMTPat (HST.ralloc_post i init h x h')]
 let modifies_ralloc_post = MG.modifies_ralloc_post #_ #cls
 
-val modifies_salloc_post
-  (#a: Type)
-  (#rel: Preorder.preorder a)
-  (init: a)
-  (h: HS.mem)
-  (x: HST.mreference a rel { HS.is_stack_region (HS.frameOf x) } )
-  (h' : HS.mem)
-: Lemma
-  (requires (HST.salloc_post init h x h'))
-  (ensures (modifies loc_none h h'))
-  [SMTPat (HST.salloc_post init h x h')]
 let modifies_salloc_post = MG.modifies_salloc_post #_ #cls
 
-/// Modifies clause for freeing a reference: the address is modified.
-
-val modifies_free
-  (#a: Type)
-  (#rel: Preorder.preorder a)
-  (r: HS.mreference a rel { HS.is_mm r } )
-  (m: HS.mem { m `HS.contains` r } )
-: Lemma
-  (modifies (loc_freed_mreference r) m (HS.free r m))
-  [SMTPat (HS.free r m)]
 let modifies_free = MG.modifies_free #_ #cls
 
-/// Another compatibility lemma
-
-val modifies_none_modifies
-  (h1 h2: HS.mem)
-: Lemma
-  (requires (HST.modifies_none h1 h2))
-  (ensures (modifies loc_none h1 h2))
-  [SMTPat (HST.modifies_none h1 h2)]
 let modifies_none_modifies = MG.modifies_none_modifies #_ #cls
 
-/// Compatibility with HS.upd
-
-val modifies_upd
-  (#t: Type) (#pre: Preorder.preorder t)
-  (r: HS.mreference t pre)
-  (v: t)
-  (h: HS.mem)
-: Lemma
-  (requires (HS.contains h r))
-  (ensures (modifies (loc_mreference r) h (HS.upd h r v)))
-  [SMTPat (HS.upd h r v)]
 let modifies_upd = MG.modifies_upd #_ #cls
 
 val modifies_0_modifies
@@ -1855,7 +729,6 @@ val modifies_0_modifies
 : Lemma
   (requires (modifies_0 h1 h2))
   (ensures (modifies loc_none h1 h2))
-
 let modifies_0_modifies h1 h2 =
   MG.modifies_none_intro #_ #cls h1 h2
     (fun r -> modifies_0_live_region h1 h2 r)
@@ -1912,452 +785,97 @@ let modifies_addr_of_modifies #t #_ #_ b h1 h2 =
       modifies_addr_of_unused_in b h1 h2 r n
     )
 
-
-///  A memory ``h`` does not contain address ``a`` in region ``r``, denoted
-///  ``does_not_contain_addr h (r, a)``, only if, either region ``r`` is
-///  not live, or address ``a`` is unused in region ``r``.
-
-(* BEGIN TODO: move to FStar.Monotonic.HyperStack *)
-
-val does_not_contain_addr
-  (h: HS.mem)
-  (ra: HS.rid * nat)
-: GTot Type0
 let does_not_contain_addr = MG.does_not_contain_addr
 
-val not_live_region_does_not_contain_addr
-  (h: HS.mem)
-  (ra: HS.rid * nat)
-: Lemma
-  (requires (~ (HS.live_region h (fst ra))))
-  (ensures (h `does_not_contain_addr` ra))
 let not_live_region_does_not_contain_addr = MG.not_live_region_does_not_contain_addr
 
-val unused_in_does_not_contain_addr
-  (h: HS.mem)
-  (#a: Type)
-  (#rel: Preorder.preorder a)
-  (r: HS.mreference a rel)
-: Lemma
-  (requires (r `HS.unused_in` h))
-  (ensures (h `does_not_contain_addr` (HS.frameOf r, HS.as_addr r)))
 let unused_in_does_not_contain_addr = MG.unused_in_does_not_contain_addr
 
-val addr_unused_in_does_not_contain_addr
-  (h: HS.mem)
-  (ra: HS.rid * nat)
-: Lemma
-  (requires (HS.live_region h (fst ra) ==> snd ra `Heap.addr_unused_in` (Map.sel (HS.get_hmap h) (fst ra))))
-  (ensures (h `does_not_contain_addr` ra))
 let addr_unused_in_does_not_contain_addr = MG.addr_unused_in_does_not_contain_addr
 
-val free_does_not_contain_addr
-  (#a: Type0)
-  (#rel: Preorder.preorder a)
-  (r: HS.mreference a rel)
-  (m: HS.mem)
-  (x: HS.rid * nat)
-: Lemma
-  (requires (
-    HS.is_mm r /\
-    m `HS.contains` r /\
-    fst x == HS.frameOf r /\
-    snd x == HS.as_addr r
-  ))
-  (ensures (
-    HS.free r m `does_not_contain_addr` x
-  ))
-  [SMTPat (HS.free r m `does_not_contain_addr` x)]
 let free_does_not_contain_addr = MG.free_does_not_contain_addr
 
-val does_not_contain_addr_elim
-  (#a: Type0)
-  (#rel: Preorder.preorder a)
-  (r: HS.mreference a rel)
-  (m: HS.mem)
-  (x: HS.rid * nat)
-: Lemma
-  (requires (
-    m `does_not_contain_addr` x /\
-    HS.frameOf r == fst x /\
-    HS.as_addr r == snd x
-  ))
-  (ensures (~ (m `HS.contains` r)))
 let does_not_contain_addr_elim = MG.does_not_contain_addr_elim
 
-(** END TODO *)
-
-/// Addresses that have not been allocated yet can be removed from
-/// modifies clauses.
-
-val modifies_only_live_addresses
-  (r: HS.rid)
-  (a: Set.set nat)
-  (l: loc)
-  (h h' : HS.mem)
-: Lemma
-  (requires (
-    modifies (loc_union (loc_addresses false r a) l) h h' /\
-    (forall x . Set.mem x a ==> h `does_not_contain_addr` (r, x))
-  ))
-  (ensures (modifies l h h'))
 let modifies_only_live_addresses = MG.modifies_only_live_addresses
 
-
-(* Generic way to ensure that a buffer just allocated is disjoint from
-   any other object, however the latter's liveness is defined. *)
-
-val loc_not_unused_in (h: HS.mem) : GTot loc
 let loc_not_unused_in = MG.loc_not_unused_in _
 
-val loc_unused_in (h: HS.mem) : GTot loc
 let loc_unused_in = MG.loc_unused_in _
 
-val loc_unused_in_not_unused_in_disjoint (h: HS.mem) : Lemma
-  (loc_disjoint (loc_unused_in h) (loc_not_unused_in h))
 let loc_unused_in_not_unused_in_disjoint =
   MG.loc_unused_in_not_unused_in_disjoint cls
 
-val not_live_region_loc_not_unused_in_disjoint
-  (h0: HS.mem)
-  (r: HS.rid)
-: Lemma
-  (requires (~ (HS.live_region h0 r)))
-  (ensures (loc_disjoint (loc_region_only false r) (loc_not_unused_in h0)))
 let not_live_region_loc_not_unused_in_disjoint = MG.not_live_region_loc_not_unused_in_disjoint cls
 
-let fresh_frame_loc_not_unused_in_disjoint
-  (h0 h1: HS.mem)
-: Lemma
-  (requires (HS.fresh_frame h0 h1))
-  (ensures (loc_disjoint (loc_region_only false (HS.get_tip h1)) (loc_not_unused_in h0)))
-  [SMTPat (HS.fresh_frame h0 h1)]
-= not_live_region_loc_not_unused_in_disjoint h0 (HS.get_tip h1)
-
-val live_loc_not_unused_in (#a:Type0) (#rrel #rel:srel a) (b:mbuffer a rrel rel) (h:HS.mem)
-  :Lemma (requires (live h b))
-         (ensures  (loc_not_unused_in h `loc_includes` loc_addr_of_buffer b))
-         [SMTPat (live h b)]
 let live_loc_not_unused_in #_ #_ #_ b h =
   unused_in_equiv b h;
   Classical.move_requires (MG.does_not_contain_addr_addr_unused_in h) (frameOf b, as_addr b);
   MG.loc_addresses_not_unused_in cls (frameOf b) (Set.singleton (as_addr b)) h;
   ()
 
-val unused_in_loc_unused_in (#a:Type0) (#rrel #rel:srel a) (b:mbuffer a rrel rel) (h:HS.mem)
-  :Lemma (requires (unused_in b h))
-         (ensures  (loc_unused_in h `loc_includes` loc_addr_of_buffer b))
-         [SMTPat (unused_in b h)]
 let unused_in_loc_unused_in #_ #_ #_ b h =
   unused_in_equiv b h;
   Classical.move_requires (MG.addr_unused_in_does_not_contain_addr h) (frameOf b, as_addr b);
   MG.loc_addresses_unused_in cls (frameOf b) (Set.singleton (as_addr b)) h;
   ()
 
-val modifies_address_liveness_insensitive_unused_in
-  (h h' : HS.mem)
-: Lemma
-  (requires (modifies (address_liveness_insensitive_locs) h h'))
-  (ensures (loc_not_unused_in h' `loc_includes` loc_not_unused_in h /\ loc_unused_in h `loc_includes` loc_unused_in h'))
 let modifies_address_liveness_insensitive_unused_in =
   MG.modifies_address_liveness_insensitive_unused_in cls
 
-/// Addresses that have not been allocated yet can be removed from
-/// modifies clauses.
-
-val modifies_only_not_unused_in
-  (l: loc)
-  (h h' : HS.mem)
-: Lemma
-  (requires (modifies (loc_union (loc_unused_in h) l) h h'))
-  (ensures (modifies l h h'))
 let modifies_only_not_unused_in = MG.modifies_only_not_unused_in
 
-val mreference_live_loc_not_unused_in
-  (#t: Type)
-  (#pre: Preorder.preorder t)
-  (h: HS.mem)
-  (r: HS.mreference t pre)
-: Lemma
-  (requires (h `HS.contains` r))
-  (ensures (loc_not_unused_in h `loc_includes` loc_freed_mreference r /\ loc_not_unused_in h `loc_includes` loc_mreference r))
-  [SMTPat (HS.contains h r)]
 let mreference_live_loc_not_unused_in =
   MG.mreference_live_loc_not_unused_in cls
 
-val mreference_unused_in_loc_unused_in
-  (#t: Type)
-  (#pre: Preorder.preorder t)
-  (h: HS.mem)
-  (r: HS.mreference t pre)
-: Lemma
-  (requires (r `HS.unused_in` h))
-  (ensures (loc_unused_in h `loc_includes` loc_freed_mreference r /\ loc_unused_in h `loc_includes` loc_mreference r))
-  [SMTPat (HS.unused_in r h)]
 let mreference_unused_in_loc_unused_in =
   MG.mreference_unused_in_loc_unused_in cls
 
-
-let unused_in_not_unused_in_disjoint_2
-  (l1 l2 l1' l2': loc)
-  (h: HS.mem)
-: Lemma
-  (requires (loc_unused_in h `loc_includes` l1 /\ loc_not_unused_in h `loc_includes` l2 /\ l1 `loc_includes` l1' /\ l2 `loc_includes` l2' ))
-  (ensures (loc_disjoint l1'  l2' ))
-  [SMTPat (loc_disjoint l1' l2'); SMTPat (loc_unused_in h `loc_includes` l1); SMTPat (loc_not_unused_in h `loc_includes` l2)]
-= loc_includes_trans (loc_unused_in h) l1 l1' ;
-  loc_includes_trans (loc_not_unused_in h) l2 l2'  ;
-  loc_unused_in_not_unused_in_disjoint h ;
-  loc_disjoint_includes (loc_unused_in h) (loc_not_unused_in h) l1' l2' 
-
-
 (* Duplicate the modifies clause to cope with cases that must not be used with transitivity *)
 
-val modifies_inert
-  (s: loc)
-  (h1 h2: HS.mem)
-: GTot Type0
 let modifies_inert = modifies
 
-val modifies_inert_intro
-  (s: loc)
-  (h1 h2: HS.mem)
-: Lemma
-  (requires (modifies s h1 h2))
-  (ensures (modifies_inert s h1 h2))
-  [SMTPat (modifies s h1 h2)]
 let modifies_inert_intro s h1 h2 = ()
 
-val modifies_inert_live_region
-  (s: loc)
-  (h1 h2: HS.mem)
-  (r: HS.rid)
-: Lemma
-  (requires (modifies_inert s h1 h2 /\ loc_disjoint s (loc_region_only false r) /\ HS.live_region h1 r))
-  (ensures (HS.live_region h2 r))
-  [SMTPatOr [
-    [SMTPat (modifies_inert s h1 h2); SMTPat (HS.live_region h1 r)];
-    [SMTPat (modifies_inert s h1 h2); SMTPat (HS.live_region h2 r)];
-  ]]
 let modifies_inert_live_region = modifies_live_region
 
-val modifies_inert_mreference_elim
-  (#t: Type)
-  (#pre: Preorder.preorder t)
-  (b: HS.mreference t pre)
-  (p: loc)
-  (h h': HS.mem)
-: Lemma
-  (requires (
-    loc_disjoint (loc_mreference b) p /\
-    HS.contains h b /\
-    modifies_inert p h h'
-  ))
-  (ensures (
-    HS.contains h' b /\
-    HS.sel h b == HS.sel h' b
-  ))
-  [SMTPatOr [
-    [ SMTPat (modifies_inert p h h'); SMTPat (HS.sel h b) ] ;
-    [ SMTPat (modifies_inert p h h'); SMTPat (HS.contains h b) ];
-    [ SMTPat (modifies_inert p h h'); SMTPat (HS.sel h' b) ] ;
-    [ SMTPat (modifies_inert p h h'); SMTPat (HS.contains h' b) ]
-  ] ]
 let modifies_inert_mreference_elim = modifies_mreference_elim
 
-val modifies_inert_buffer_elim (#a:Type0) (#rrel #rel:srel a)
-  (b:mbuffer a rrel rel)
-  (p:loc)
-  (h h':HS.mem)
-  :Lemma (requires (loc_disjoint (loc_buffer b) p /\
-                    live h b /\
-                    modifies_inert p h h'))
-         (ensures  (live h' b /\ (as_seq h b == as_seq h' b)))
-         [SMTPatOr [
-             [ SMTPat (modifies_inert p h h'); SMTPat (as_seq h b) ] ;
-             [ SMTPat (modifies_inert p h h'); SMTPat (live h b) ];
-             [ SMTPat (modifies_inert p h h'); SMTPat (as_seq h' b) ] ;
-             [ SMTPat (modifies_inert p h h'); SMTPat (live h' b) ]
-         ] ]
 let modifies_inert_buffer_elim = modifies_buffer_elim
 
-val modifies_inert_liveness_insensitive_mreference_weak
-  (l : loc)
-  (h h' : HS.mem)
-  (#t: Type)
-  (#pre: Preorder.preorder t)
-  (x: HS.mreference t pre)
-: Lemma
-  (requires (modifies_inert l h h' /\ address_liveness_insensitive_locs `loc_includes` l /\ h `HS.contains` x))
-  (ensures (h' `HS.contains` x))
-  [SMTPatOr [
-    [SMTPat (h `HS.contains` x); SMTPat (modifies_inert l h h');];
-    [SMTPat (h' `HS.contains` x); SMTPat (modifies_inert l h h');];
-  ]]
 let modifies_inert_liveness_insensitive_mreference_weak = modifies_liveness_insensitive_mreference_weak
 
-val modifies_inert_liveness_insensitive_buffer_weak
-  (l:loc)
-  (h h':HS.mem)
-  (#a:Type0) (#rrel #rel:srel a)
-  (x:mbuffer a rrel rel)
-  :Lemma (requires (modifies_inert l h h' /\ address_liveness_insensitive_locs `loc_includes` l /\ live h x))
-         (ensures (live h' x))
-         [SMTPatOr [
-             [SMTPat (live h x); SMTPat (modifies_inert l h h');];
-             [SMTPat (live h' x); SMTPat (modifies_inert l h h');];
-         ]]
 let modifies_inert_liveness_insensitive_buffer_weak = modifies_liveness_insensitive_buffer_weak
 
-val modifies_inert_liveness_insensitive_region_weak
-  (l2 : loc)
-  (h h' : HS.mem)
-  (x: HS.rid)
-: Lemma
-  (requires (modifies_inert l2 h h' /\ region_liveness_insensitive_locs `loc_includes` l2 /\ HS.live_region h x))
-  (ensures (HS.live_region h' x))
-  [SMTPatOr [
-    [SMTPat (modifies_inert l2 h h'); SMTPat (HS.live_region h x)];
-    [SMTPat (modifies_inert l2 h h'); SMTPat (HS.live_region h' x)];
-  ]]
 let modifies_inert_liveness_insensitive_region_weak = modifies_liveness_insensitive_region_weak
 
-val modifies_inert_liveness_insensitive_region_mreference_weak
-  (l2 : loc)
-  (h h' : HS.mem)
-  (#t: Type)
-  (#pre: Preorder.preorder t)
-  (x: HS.mreference t pre)
-: Lemma
-  (requires (modifies_inert l2 h h' /\ region_liveness_insensitive_locs `loc_includes` l2 /\ HS.live_region h (HS.frameOf x)))
-  (ensures (HS.live_region h' (HS.frameOf x)))
-  [SMTPatOr [
-    [SMTPat (modifies_inert l2 h h'); SMTPat (HS.live_region h (HS.frameOf x))];
-    [SMTPat (modifies_inert l2 h h'); SMTPat (HS.live_region h' (HS.frameOf x))];
-  ]]
 let modifies_inert_liveness_insensitive_region_mreference_weak = modifies_liveness_insensitive_region_mreference_weak
 
-val modifies_inert_liveness_insensitive_region_buffer_weak
-  (l2:loc)
-  (h h':HS.mem)
-  (#a:Type0) (#rrel #rel:srel a)
-  (x:mbuffer a rrel rel)
-  :Lemma (requires (modifies_inert l2 h h' /\ region_liveness_insensitive_locs `loc_includes` l2 /\ HS.live_region h (frameOf x)))
-         (ensures  (HS.live_region h' (frameOf x)))
-         [SMTPatOr [
-             [SMTPat (modifies_inert l2 h h'); SMTPat (HS.live_region h (frameOf x))];
-             [SMTPat (modifies_inert l2 h h'); SMTPat (HS.live_region h' (frameOf x))];
-         ]]
 let modifies_inert_liveness_insensitive_region_buffer_weak = modifies_liveness_insensitive_region_buffer_weak
 
-val fresh_frame_modifies_inert
-  (h0 h1: HS.mem)
-: Lemma
-  (requires (HS.fresh_frame h0 h1))
-  (ensures (modifies_inert loc_none h0 h1))
-  [SMTPat (HS.fresh_frame h0 h1)]
 let fresh_frame_modifies_inert = fresh_frame_modifies
 
-val popped_modifies_inert
-  (h0 h1: HS.mem)
-: Lemma
-  (requires (HS.popped h0 h1))
-  (ensures (modifies_inert (loc_region_only false (HS.get_tip h0)) h0 h1))
-  [SMTPat (HS.popped h0 h1)]
 let popped_modifies_inert = popped_modifies
 
-val modifies_inert_loc_unused_in
-  (l: loc)
-  (h1 h2: HS.mem)
-  (l' : loc)
-: Lemma
-  (requires (
-    modifies_inert l h1 h2 /\
-    address_liveness_insensitive_locs `loc_includes` l /\
-    loc_unused_in h2 `loc_includes` l'
-  ))
-  (ensures (loc_unused_in h1 `loc_includes` l'))
-  [SMTPat (modifies_inert l h1 h2); SMTPat (loc_unused_in h2 `loc_includes` l')]
 let modifies_inert_loc_unused_in l h1 h2 l' =
   modifies_loc_includes address_liveness_insensitive_locs h1 h2 l;
   modifies_address_liveness_insensitive_unused_in h1 h2;
   loc_includes_trans (loc_unused_in h1) (loc_unused_in h2) l'
 
-/// Legacy shorthands for disjointness and inclusion of buffers
-///
-let disjoint (#a1 #a2:Type0) (#rrel1 #rel1:srel a1) (#rrel2 #rel2:srel a2)
-  (b1:mbuffer a1 rrel1 rel1) (b2:mbuffer a2 rrel2 rel2) :GTot Type0 =
-  loc_disjoint (loc_buffer b1) (loc_buffer b2)
-
-let includes (#a1 #a2:Type0) (#rrel1 #rel1:srel a1) (#rrel2 #rel2:srel a2)
-  (b1:mbuffer a1 rrel1 rel1) (b2:mbuffer a2 rrel2 rel2) :GTot Type0 =
-  loc_includes (loc_buffer b1) (loc_buffer b2) /\
-  (g_is_null b1 <==> g_is_null b2)
-
-val disjoint_neq (#a1 #a2:Type0) (#rrel1 #rel1:srel a1) (#rrel2 #rel2:srel a2)
-  (b1:mbuffer a1 rrel1 rel1) (b2:mbuffer a2 rrel2 rel2)
-  :Lemma (requires (disjoint b1 b2 /\ U32.v (len b1) > 0))
-         (ensures (~(b1 === b2)))
 let disjoint_neq #_ #_ #_ #_ #_ #_ b1 b2 =
-  if frameOf b1 = frameOf b2 && as_addr b1 = as_addr b2
-  then
+  if frameOf b1 = frameOf b2 && as_addr b1 = as_addr b2 then
     MG.loc_disjoint_aloc_elim #_ #cls #(frameOf b1) #(as_addr b1) #(frameOf b2) #(as_addr b2) (ubuffer_of_buffer b1) (ubuffer_of_buffer b2)
   else ()
-
-/// The liveness of a sub-buffer is exactly equivalent to the liveness
-/// of its enclosing buffer.
-
-val includes_live (#a:Type0) (#rrel #rel1 #rel2:srel a)
-  (h:HS.mem) (larger:mbuffer a rrel rel1) (smaller:mbuffer a rrel rel2)
-  :Lemma (requires (larger `includes` smaller))
-         (ensures  (live h larger <==> live h smaller))
-         [SMTPatOr [
-             [SMTPat (includes larger smaller); SMTPat (live h larger)];
-             [SMTPat (includes larger smaller); SMTPat (live h smaller)];
-         ]]
 let includes_live #a #rrel #rel1 #rel2 h larger smaller =
-  if Null? larger || Null? smaller
-  then ()
+  if Null? larger || Null? smaller then ()
   else
     MG.loc_includes_aloc_elim #_ #cls #(frameOf larger) #(frameOf smaller) #(as_addr larger) #(as_addr smaller) (ubuffer_of_buffer larger) (ubuffer_of_buffer smaller)
 
-val includes_frameOf_as_addr (#a1 #a2:Type0) (#rrel1 #rel1:srel a1) (#rrel2 #rel2:srel a2)
-  (larger:mbuffer a1 rrel1 rel1) (smaller:mbuffer a2 rrel2 rel2)
-  :Lemma (requires (larger `includes` smaller))
-         (ensures (g_is_null larger == g_is_null smaller /\ frameOf larger == frameOf smaller /\ as_addr larger == as_addr smaller))
-         [SMTPat (larger `includes` smaller)]
 let includes_frameOf_as_addr #_ #_ #_ #_ #_ #_ larger smaller =
-  if Null? larger || Null? smaller
-  then ()
+  if Null? larger || Null? smaller then ()
   else
     MG.loc_includes_aloc_elim #_ #cls #(frameOf larger) #(frameOf smaller) #(as_addr larger) #(as_addr smaller) (ubuffer_of_buffer larger) (ubuffer_of_buffer smaller)
 
-
-/// 
-/// Useful shorthands for pointers, or maybe-null pointers
-
-inline_for_extraction
-type mpointer (a:Type0) (rrel:srel a) (rel:srel a)  =
-  b:mbuffer a rrel rel{length b == 1}
-
-inline_for_extraction
-type mpointer_or_null (a:Type0) (rrel:srel a) (rel:srel a) =
-  b:mbuffer a rrel rel{if g_is_null b then True else length b == 1}
-
-unfold
-let deref (#a:Type0) (#rrel #rel:srel a) (h:HS.mem) (x:mpointer a rrel rel) =
-  get h x 0
-
-/// Two pointers having different contents are disjoint. This is valid
-/// only for pointers, i.e. buffers of size 1.
-
-val pointer_distinct_sel_disjoint
-  (#a:Type0) (#rrel1 #rrel2 #rel1 #rel2:srel a)
-  (b1:mpointer a rrel1 rel1)
-  (b2:mpointer a rrel2 rel2)
-  (h:HS.mem)
-  :Lemma (requires (live h b1 /\ live h b2 /\ get h b1 0 =!= get h b2 0))
-         (ensures  (disjoint b1 b2))
 let pointer_distinct_sel_disjoint #a #_ #_ #_ #_ b1 b2 h =
   if frameOf b1 = frameOf b2 && as_addr b1 = as_addr b2
   then begin
@@ -2367,89 +885,34 @@ let pointer_distinct_sel_disjoint #a #_ #_ #_ #_ b1 b2 h =
   else
     loc_disjoint_buffer b1 b2
 	 
-/// The following stateful operations on buffers do not change the
-/// memory, but, as required by the C standard, they all require the
-/// buffer in question to be live.
-
-/// The nullity test, ``is_null b``, which KreMLin compiles to C as ``b == NULL``.
-
-val is_null (#a:Type0) (#rrel #rel:srel a) (b:mbuffer a rrel rel)
-  :HST.Stack bool (requires (fun h -> live h b))
-                  (ensures  (fun h y h' -> h == h' /\ y == g_is_null b))
 let is_null #_ #_ #_ b = Null? b
 
-/// ``sub b i len`` constructs the sub-buffer of ``b`` starting from
-/// offset ``i`` with length ``len``. KreMLin extracts this operation as
-/// ``b + i`` (or, equivalently, ``&b[i]``.)
-
-val sub (#a:Type0) (#rrel #rel:srel a) (b:mbuffer a rrel rel)
-  (i:U32.t) (len:U32.t) (sub_rel:srel a)
-  :HST.Stack (mbuffer a rrel sub_rel)
-             (requires (fun h -> U32.v i + U32.v len <= length b /\ compatible_sub b i len sub_rel /\ live h b))
-             (ensures  (fun h y h' -> h == h' /\ y == gsub b i len sub_rel))
 let sub #a #rrel #rel b i len sub_rel =
   match b with
   | Null -> Null
   | Buffer max_len content i0 len0 () ->
-    lemma_sub_compatibility_is_transitive (U32.v max_len) rrel (U32.v i0) (U32.v len0) rel (U32.v i) (U32.v len) sub_rel;
+    Seq.lemma_seq_sub_compatibility_is_transitive (U32.v max_len) rrel (U32.v i0) (U32.v i0 + U32.v len0) rel
+                                                  (U32.v i) (U32.v i + U32.v len) sub_rel;
     Buffer max_len content (U32.add i0 i) len ()
 
-/// ``offset b i`` construct the tail of the buffer ``b`` starting from
-/// offset ``i``, i.e. the sub-buffer of ``b`` starting from offset ``i``
-/// with length ``U32.sub (len b) i``. KreMLin compiles it as ``b + i`` or
-/// ``&b[i]``.
-///
-/// This stateful operation cannot be derived from ``sub``, because the
-/// length cannot be computed outside of proofs.
-
-val offset (#a:Type0) (#rrel #rel:srel a) (b:mbuffer a rrel rel)
-  (i:U32.t) (sub_rel:srel a)
-  :HST.Stack (mbuffer a rrel sub_rel)
-             (requires (fun h -> U32.v i <= length b /\ compatible_sub b i (U32.sub (len b) i) sub_rel /\ live h b))
-             (ensures  (fun h y h' -> h == h' /\ y == gsub b i (U32.sub (len b) i) sub_rel))
 let offset #a #rrel #rel b i sub_rel =
   match b with
   | Null -> Null
   | Buffer max_len content i0 len () ->
-    lemma_sub_compatibility_is_transitive (U32.v max_len) rrel (U32.v i0) (U32.v len) rel (U32.v i) (U32.v (U32.sub len i)) sub_rel;
+    Seq.lemma_seq_sub_compatibility_is_transitive (U32.v max_len) rrel (U32.v i0) (U32.v i0 + U32.v len) rel
+                                                  (U32.v i) (U32.v i + U32.v (U32.sub len i)) sub_rel;
     Buffer max_len content (U32.add i0 i) (U32.sub len i) ()
 
-/// ``index b i`` reads the value of ``b`` at offset ``i`` from memory and
-/// returns it. KreMLin compiles it as b[i].
-val index (#a:Type0)(#rrel #rel:srel a) (b:mbuffer a rrel rel) (i:U32.t)
-  :HST.Stack a (requires (fun h -> live h b /\ U32.v i < length b))
-               (ensures  (fun h y h' -> h == h' /\ y == Seq.index (as_seq h b) (U32.v i)))
 let index #_ #_ #_ b i =
   let open HST in
   let s = ! (Buffer?.content b) in
   Seq.index s (U32.v (Buffer?.idx b) + U32.v i)
-
-/// The following stateful operations on buffers modify the memory,
-/// and, as usual, require the liveness of the buffer.
-
-/// ``g_upd_seq b s h`` updates the entire buffer `b`'s contents in
-/// heap `h` to correspond to the sequence `s`
-val g_upd_seq (#a:Type0) (#rrel #rel:srel a)
-              (b:mbuffer a rrel rel) (s:Seq.lseq a (length b))
-	      (h:HS.mem{live h b /\ rel (as_seq h b) s})
-  :GTot HS.mem
 let g_upd_seq #_ #_ #_ b s h =
   if Seq.length s = 0 then h
   else
     let s0 = HS.sel h (Buffer?.content b) in
     HS.upd h (Buffer?.content b) (replace_subseq s0 (U32.v (Buffer?.idx b)) (length b) s)
 
-/// A lemma specifying `g_upd_seq` in terms of its effect on the
-/// buffer's underlying sequence
-val g_upd_seq_as_seq (#a:Type0) (#rrel #rel:srel a)
-                     (b:mbuffer a rrel rel)
-                     (s:Seq.lseq a (length b))
-                     (h:HS.mem{live h b /\ rel (as_seq h b) s})
-  : Lemma (let h' = g_upd_seq b s h in
-           (Seq.length s > 0 ==> not (g_is_null b)) /\
-           modifies (loc_buffer b) h h' /\
-           live h' b /\
-           as_seq h' b == s)
 #push-options "--z3rlimit 32"
 let g_upd_seq_as_seq #_ #_ #_ b s h =
   let h' = g_upd_seq b s h in
@@ -2464,29 +927,6 @@ let g_upd_seq_as_seq #_ #_ #_ b s h =
   end
 #pop-options
 
-
-/// ``g_upd b i v h`` updates the buffer `b` in heap `h` at location
-/// `i` writing ``v`` there. This is the spec analog of the stateful
-/// update `upd` below.
-let g_upd (#a:Type0) (#rrel #rel:srel a)
-          (b:mbuffer a rrel rel)
-          (i:nat{i < length b})
-          (v:a)
-          (h:HS.mem{live h b /\ rel (as_seq h b) (Seq.upd (as_seq h b) i v)})
-  : GTot HS.mem
-  = g_upd_seq b (Seq.upd (as_seq h b) i v) h
-
-/// ``upd b i v`` writes ``v`` to the memory, at offset ``i`` of
-/// buffer ``b``. KreMLin compiles it as ``b[i] = v``.
-
-val upd'
-  (#a:Type0) (#rrel #rel:srel a)
-  (b:mbuffer a rrel rel)
-  (i:U32.t)
-  (v:a)
-  :HST.Stack unit (requires (fun h -> live h b /\ U32.v i < length b /\
-                                   rel (as_seq h b) (Seq.upd (as_seq h b) (U32.v i) v)))
-                  (ensures  (fun h _ h' -> h' == g_upd b (U32.v i) v h))
 let upd' #_ #_ #_ b i v =
   let open HST in
   let Buffer max_length content idx len () = b in
@@ -2494,122 +934,35 @@ let upd' #_ #_ #_ b i v =
   let sb0 = Seq.slice s0 (U32.v idx) (U32.v idx + U32.v len) in
   Buffer?.content b := replace_subseq s0 (U32.v idx) (U32.v len) (Seq.upd sb0 (U32.v i) v)
 
-inline_for_extraction
-let upd
-  (#a:Type0) (#rrel #rel:srel a)
-  (b:mbuffer a rrel rel)
-  (i:U32.t)
-  (v:a)
-  : HST.Stack unit (requires (fun h -> live h b /\ U32.v i < length b /\ 
-                                    rel (as_seq h b) (Seq.upd (as_seq h b) (U32.v i) v)))
-                   (ensures (fun h _ h' -> (not (g_is_null b)) /\
-                                        modifies (loc_buffer b) h h' /\
-                                        live h' b /\
-                                        as_seq h' b == Seq.upd (as_seq h b) (U32.v i) v))
-  = let h = HST.get () in
-    upd' b i v;
-    g_upd_seq_as_seq b (Seq.upd (as_seq h b) (U32.v i) v) h
-
-val recallable (#a:Type0) (#rrel #rel:srel a) (b:mbuffer a rrel rel) :GTot Type0
-let recallable' (#a:Type0) (#rrel #rel:srel a) (b:mbuffer a rrel rel) :GTot Type0 =
+let recallable (#a:Type0) (#rrel #rel:srel a) (b:mbuffer a rrel rel) :GTot Type0 =
   (not (g_is_null b)) ==> (
     HST.is_eternal_region (frameOf b) /\
-    not (HS.is_mm (Buffer?.content b))
-  )
+    not (HS.is_mm (Buffer?.content b)))
 
-let recallable = recallable'
-
-(* TODO: candidate for wrapper *)
-val recallable_null (#a:Type0) (#rrel #rel:srel a)
-  :Lemma (recallable (null #a #rrel #rel)) [SMTPat (recallable (null #a #rrel #rel))]
 let recallable_null #_ #_ #_ = ()
 
-val recallable_includes (#a1 #a2:Type0) (#rrel1 #rel1:srel a1) (#rrel2 #rel2:srel a2)
-  (larger:mbuffer a1 rrel1 rel1) (smaller:mbuffer a2 rrel2 rel2)
-  :Lemma (requires (larger `includes` smaller))
-         (ensures (recallable larger <==> recallable smaller))
-         [SMTPatOr [
-             [SMTPat (recallable larger); SMTPat (recallable smaller);];
-             [SMTPat (larger `includes` smaller)];
-         ]]
 let recallable_includes #_ #_ #_ #_ #_ #_ larger smaller =
   if Null? larger || Null? smaller then ()
   else
     MG.loc_includes_aloc_elim #_ #cls #(frameOf larger) #(frameOf smaller) #(as_addr larger) #(as_addr smaller) (ubuffer_of_buffer larger) (ubuffer_of_buffer smaller)
 
-val recall (#a:Type0) (#rrel #rel:srel a) (b:mbuffer a rrel rel)
-  :HST.Stack unit (requires (fun _ -> recallable b))
-                  (ensures  (fun m0 _ m1 -> m0 == m1 /\ live m1 b))
-let recall #_ #_ #_ b =
-  if Null? b then ()
-  else HST.recall (Buffer?.content b)
+let recall #_ #_ #_ b = if Null? b then () else HST.recall (Buffer?.content b)
 
-
-/// Deallocation. A buffer that was allocated by ``malloc`` (see below)
-/// can be ``free`` d.
-
-val freeable (#a:Type0) (#rrel #rel:srel a) (b:mbuffer a rrel rel) :GTot Type0
-let freeable' (#a:Type0) (#rrel #rel:srel a) (b:mbuffer a rrel rel) =
+let freeable (#a:Type0) (#rrel #rel:srel a) (b:mbuffer a rrel rel) =
   (not (g_is_null b)) /\
   HS.is_mm (Buffer?.content b) /\
   HST.is_eternal_region (frameOf b) /\
   U32.v (Buffer?.max_length b) > 0 /\
   Buffer?.idx b == 0ul /\
   Buffer?.length b == Buffer?.max_length b
-let freeable = freeable'
 
-val free (#a:Type0) (#rrel #rel:srel a) (b:mbuffer a rrel rel)
-  :HST.ST unit (requires (fun h0 -> live h0 b /\ freeable b))
-               (ensures  (fun h0 _ h1 -> (not (g_is_null b)) /\
-                                      Map.domain (HS.get_hmap h1) `Set.equal` Map.domain (HS.get_hmap h0) /\ 
-                                      (HS.get_tip h1) == (HS.get_tip h0) /\
-                                      modifies (loc_addr_of_buffer b) h0 h1 /\
-                                      HS.live_region h1 (frameOf b)))
 let free #_ #_ #_ b = HST.rfree (Buffer?.content b)
 
-val freeable_length (#a:Type0) (#rrel #rel:srel a) (b:mbuffer a rrel rel)
-  :Lemma (requires (freeable b)) (ensures (length b > 0))
-         [SMTPat (freeable b)]
 let freeable_length #_ #_ #_ b = ()
 
-val freeable_disjoint (#a1 #a2:Type0) (#rrel1 #rel1:srel a1) (#rrel2 #rel2:srel a2)
-  (b1:mbuffer a1 rrel1 rel1) (b2:mbuffer a2 rrel2 rel2)
-  :Lemma (requires (freeable b1 /\ length b2 > 0 /\ disjoint b1 b2))
-         (ensures (frameOf b1 <> frameOf b2 \/ as_addr b1 <> as_addr b2))
 let freeable_disjoint #_ #_ #_ #_ #_ #_ b1 b2 =
-  if frameOf b1 = frameOf b2 && as_addr b1 = as_addr b2
-  then
+  if frameOf b1 = frameOf b2 && as_addr b1 = as_addr b2 then
     MG.loc_disjoint_aloc_elim #_ #cls #(frameOf b1) #(as_addr b1) #(frameOf b2) #(as_addr b2) (ubuffer_of_buffer b1) (ubuffer_of_buffer b2)
-  else ()
-
-let freeable_disjoint' (#a1 #a2:Type0) (#rrel1 #rel1:srel a1) (#rrel2 #rel2:srel a2)
-  (b1:mbuffer a1 rrel1 rel1) (b2:mbuffer a2 rrel2 rel2)
-  :Lemma (requires (freeable b1 /\ length b2 > 0 /\ disjoint b1 b2))
-         (ensures (loc_disjoint (loc_addr_of_buffer b1) (loc_addr_of_buffer b2)))
-         [SMTPat (freeable b1); SMTPat (disjoint b1 b2)]
-  = freeable_disjoint b1 b2
-
-
-/// Allocation. This is the common postcondition of all allocation
-/// operators, which tells that the resulting buffer is fresh, and
-/// specifies its initial contents.
-
-unfold
-let alloc_post_static (#a:Type0) (#rrel #rel:srel a)
-  (r:HS.rid) (len:nat) (b:mbuffer a rrel rel)
-  = (not (g_is_null b)) /\
-    frameOf b == r /\
-    length b == len
-
-unfold
-let alloc_post_common (#a:Type0) (#rrel #rel:srel a)
-  (r:HS.rid) (len:nat) (b:mbuffer a rrel rel) (h0 h1:HS.mem)
-  = alloc_post_static r len b /\
-    b `unused_in` h0 /\
-    live h1 b /\
-    Map.domain (HS.get_hmap h1) `Set.equal` Map.domain (HS.get_hmap h0) /\ 
-    (HS.get_tip h1) == (HS.get_tip h0) /\
-    modifies loc_none h0 h1
 
 let alloc_common (#a:Type0) (#rrel:srel a)
   (r:HS.rid) (init:a) (len:U32.t) (mm:bool)
@@ -2621,141 +974,44 @@ let alloc_common (#a:Type0) (#rrel:srel a)
                                  Buffer?.idx b == 0ul /\
                                  Buffer?.length b == Buffer?.max_length b))
   = let s = Seq.create (U32.v len) init in
-    lemma_sub_compatilibity_is_reflexive (U32.v len) rrel;
+    Seq.lemma_seq_sub_compatilibity_is_reflexive (U32.v len) rrel;
     let content: HST.mreference (Seq.lseq a (U32.v len)) (srel_to_lsrel (U32.v len) rrel) =
       if mm then HST.ralloc_mm r s else HST.ralloc r s
     in
     let b = Buffer len content 0ul len () in
     b
 
-/// ``gcmalloc r init len`` allocates a memory-managed buffer of some
-/// positive length ``len`` in an eternal region ``r``. Every cell of this
-/// buffer will have initial contents ``init``. Such a buffer cannot be
-/// freed. In fact, it is eternal: it cannot be deallocated at all.
-
-(* TODO: add a wrapper AND any reason that some post is in the refinement of the return type? *)
-val gcmalloc (#a:Type0) (#rrel:srel a)
-  (r:HS.rid) (init:a) (len:U32.t)
-  :HST.ST (b:mbuffer a rrel rrel{recallable b /\ alloc_post_static r (U32.v len) b})
-          (requires (fun h -> HST.is_eternal_region r /\ U32.v len > 0))
-          (ensures  (fun h b h' -> alloc_post_common r (U32.v len) b h h' /\
-                                 as_seq h' b == Seq.create (U32.v len) init))
 let gcmalloc #_ #_ r init len = alloc_common r init len false
 
-
-/// ``malloc r init len`` allocates a hand-managed buffer of some
-/// positive length ``len`` in an eternal region ``r``. Every cell of this
-/// buffer will have initial contents ``init``. Such a buffer can be
-/// freed using ``free`` above. Note that the ``freeable`` permission is
-/// only on the whole buffer ``b``, and is not inherited by any of its
-/// strict sub-buffers.
-
-val malloc (#a:Type0) (#rrel:srel a)
-  (r:HS.rid) (init:a) (len:U32.t)
-  :HST.ST (mbuffer a rrel rrel)
-          (requires (fun h -> HST.is_eternal_region r /\ U32.v len > 0))
-          (ensures (fun h b h' -> alloc_post_common r (U32.v len) b h h' /\
-                                as_seq h' b == Seq.create (U32.v len) init /\     
-                                freeable b))
 let malloc #_ #_ r init len = alloc_common r init len true
 
-
-/// ``alloca init len`` allocates a buffer of some positive length ``len``
-/// in the current stack frame. Every cell of this buffer will have
-/// initial contents ``init``. Such a buffer cannot be freed
-/// individually, but is automatically freed as soon as its stack
-/// frame is deallocated by ``HST.pop_frame``.
-
-val alloca (#a:Type0) (#rrel:srel a)
-  (init:a) (len:U32.t)
-  :HST.StackInline (mbuffer a rrel rrel)
-                   (requires (fun h -> U32.v len > 0))
-                   (ensures (fun h b h' -> alloc_post_common (HS.get_tip h) (U32.v len) b h h' /\
-                                         as_seq h' b == Seq.create (U32.v len) init))
 let alloca #a #rrel init len =
-  lemma_sub_compatilibity_is_reflexive (U32.v len) rrel;
+  Seq.lemma_seq_sub_compatilibity_is_reflexive (U32.v len) rrel;
   let content: HST.mreference (Seq.lseq a (U32.v len)) (srel_to_lsrel (U32.v len) rrel) =
     HST.salloc (Seq.create (U32.v len) init)
   in
   let b = Buffer len content 0ul len () in
   b
 
-
-/// ``alloca_of_list init`` allocates a buffer in the current stack
-/// frame. The initial values of the cells of this buffer are
-/// specified by the ``init`` list, which must be nonempty, and of
-/// length representable as a machine integer.
-
-unfold let alloc_of_list_pre (#a:Type0) (init:list a) :GTot Type0 =
-  normalize (0 < FStar.List.Tot.length init) /\
-  normalize (FStar.List.Tot.length init <= UInt.max_int 32)
-
-unfold let alloc_of_list_post (#a:Type0) (#rrel #rel:srel a) (len:nat) (buf:mbuffer a rrel rel) :GTot Type0 =
-  normalize (length buf == len)
-
-val alloca_of_list (#a:Type0) (#rrel:srel a) (init: list a)
-  :HST.StackInline (mbuffer a rrel rrel) (requires (fun h -> alloc_of_list_pre #a init))
-                                         (ensures (fun h b h' -> let len = FStar.List.Tot.length init in
-                                                               alloc_post_common (HS.get_tip h) len b h h' /\
-                                                               as_seq h' b == Seq.seq_of_list init /\
-                                                               alloc_of_list_post #a len b))
 let alloca_of_list #a #rrel init =
   let len = U32.uint_to_t (FStar.List.Tot.length init) in
   let s = Seq.seq_of_list init in
-  lemma_sub_compatilibity_is_reflexive (U32.v len) rrel;
+  Seq.lemma_seq_sub_compatilibity_is_reflexive (U32.v len) rrel;
   let content: HST.mreference (Seq.lseq a (U32.v len)) (srel_to_lsrel (U32.v len) rrel) =
     HST.salloc s
   in
   let b = Buffer len content 0ul len () in
   b
 
-unfold let gcmalloc_of_list_pre (#a:Type0) (init:list a) :GTot Type0 =
-  normalize (FStar.List.Tot.length init <= UInt.max_int 32)
-
-(* TODO: Why is some of the post on the refinement? *)
-val gcmalloc_of_list (#a:Type0) (#rrel:srel a) (r:HS.rid) (init:list a)
-  :HST.ST (b:mbuffer a rrel rrel {
-    let len = FStar.List.Tot.length init in
-    recallable b /\
-    alloc_post_static r len b /\
-    alloc_of_list_post len b
-  })
-          (requires (fun h -> HST.is_eternal_region r /\ gcmalloc_of_list_pre #a init))
-          (ensures  (fun h b h' -> let len = FStar.List.Tot.length init in
-                                 alloc_post_common r len b h h' /\
-                                 as_seq h' b == Seq.seq_of_list init))
 let gcmalloc_of_list #a #rrel r init =
   let len = U32.uint_to_t (FStar.List.Tot.length init) in
   let s = Seq.seq_of_list init in
-  lemma_sub_compatilibity_is_reflexive (U32.v len) rrel;
+  Seq.lemma_seq_sub_compatilibity_is_reflexive (U32.v len) rrel;
   let content: HST.mreference (Seq.lseq a (U32.v len)) (srel_to_lsrel (U32.v len) rrel) =
     HST.ralloc r s
   in
   let b = Buffer len content 0ul len () in
   b
-
-/// Derived operations
-
-val blit (#a:Type0) (#rrel1 #rrel2 #rel1 #rel2:srel a)
-  (src:mbuffer a rrel1 rel1)
-  (idx_src:U32.t)
-  (dst:mbuffer a rrel2 rel2)
-  (idx_dst:U32.t)
-  (len:U32.t)
-  :HST.Stack unit (requires (fun h -> live h src /\ live h dst /\ disjoint src dst /\
-                                    U32.v idx_src + U32.v len <= length src /\
-                                    U32.v idx_dst + U32.v len <= length dst /\
-				    rel2 (as_seq h dst)
-				         (replace_subseq (as_seq h dst) (U32.v idx_dst) (U32.v len)
-					                 (mslice (as_seq h src) (U32.v idx_src) (U32.v len)))))
-                  (ensures (fun h _ h' -> modifies (loc_buffer dst) h h' /\
-                                        live h' dst /\
-                                        Seq.slice (as_seq h' dst) (U32.v idx_dst) (U32.v idx_dst + U32.v len) ==
-                                        Seq.slice (as_seq h src) (U32.v idx_src) (U32.v idx_src + U32.v len) /\
-                                        Seq.slice (as_seq h' dst) 0 (U32.v idx_dst) ==
-                                        Seq.slice (as_seq h dst) 0 (U32.v idx_dst) /\
-                                        Seq.slice (as_seq h' dst) (U32.v idx_dst + U32.v len) (length dst) ==
-                                        Seq.slice (as_seq h dst) (U32.v idx_dst + U32.v len) (length dst)))
 
 #push-options "--z3rlimit 10 --max_fuel 1 --max_ifuel 1 --initial_fuel 1 --initial_ifuel 1"
 let blit #a #rrel1 #rrel2 #rel1 #rel2 src idx_src dst idx_dst len =
@@ -2767,107 +1023,47 @@ let blit #a #rrel1 #rrel2 #rel1 #rel2 src idx_src dst idx_dst len =
     let Buffer _ content2 idx2 length2 () = dst in
     let s_full1 = !content1 in
     let s_full2 = !content2 in
-    let s1 = mslice s_full1 (U32.v idx1) (U32.v length1) in
-    let s2 = mslice s_full2 (U32.v idx2) (U32.v length2) in
-    let s_sub_src = mslice s1 (U32.v idx_src) (U32.v len) in
+    let s1 = Seq.slice s_full1 (U32.v idx1) (U32.v idx1 + U32.v length1) in
+    let s2 = Seq.slice s_full2 (U32.v idx2) (U32.v idx2 + U32.v length2) in
+    let s_sub_src = Seq.slice s1 (U32.v idx_src) (U32.v idx_src + U32.v len) in
     let s2' = replace_subseq s2 (U32.v idx_dst) (U32.v len) s_sub_src in
     let s_full2' = replace_subseq s_full2 (U32.v idx2) (U32.v length2) s2' in
     content2 := s_full2';
-    g_upd_seq_as_seq dst s2' h;
-    lemma_replace_subseq_elim s2 (U32.v idx_dst) (U32.v len) s_sub_src
+    g_upd_seq_as_seq dst s2' h
 #pop-options
-
-module L = FStar.List.Tot
-
-unfold
-let assign_list_t (#a:Type0) (#rrel #rel:srel a) (l:list a) =
-  (b:mbuffer a rrel rel) ->
-  HST.Stack unit (requires (fun h0 -> live h0 b /\
-                                    length b = L.length l /\
-				    rel (as_seq h0 b) (Seq.seq_of_list l)))
-                 (ensures (fun h0 _ h1 -> live h1 b /\
-                                        modifies (loc_buffer b) h0 h1 /\
-                                        as_seq h1 b == Seq.seq_of_list l))
-
-let assign_list (#a:Type0) (#rrel #rel:srel a) (l:list a) :assign_list_t #a #rrel #rel l
-  = fun b ->
-    let open HST in
-    if L.length l > 0 then
-      let h = get () in
-      let Buffer _ content id len () = b in
-      let s_full = !content in
-      let s_full = replace_subseq s_full (U32.v id) (U32.v len) (Seq.seq_of_list l) in
-      content := s_full;
-      g_upd_seq_as_seq b (Seq.seq_of_list l) h  //for modifies clause
-
-/// Type class instantiation for compositionality with other kinds of memory locations than regions, references or buffers (just in case).
-/// No usage pattern has been found yet.
 
 module MG = FStar.ModifiesGen
 
-val abuffer' (region: HS.rid) (addr: nat) : Tot Type0
 let abuffer' = ubuffer'
-
-inline_for_extraction
-let abuffer (region: HS.rid) (addr: nat) : Tot Type0 = G.erased (abuffer' region addr)
 
 let coerce (t2: Type) (#t1: Type) (x1: t1) : Pure t2 (requires (t1 == t2)) (ensures (fun y -> y == x1)) = x1
 
-val cloc_cls: MG.cls abuffer
 let cloc_cls =
   assert_norm (MG.cls abuffer == MG.cls ubuffer);
   coerce (MG.cls abuffer) cls
 
-val cloc_of_loc (l: loc) : Tot (MG.loc cloc_cls)
 let cloc_of_loc l =
   assert_norm (MG.cls abuffer == MG.cls ubuffer);
   coerce (MG.loc cloc_cls) l
 
-val loc_of_cloc (l: MG.loc cloc_cls) : Tot loc
 let loc_of_cloc l =
   assert_norm (MG.cls abuffer == MG.cls ubuffer);
   coerce loc l
 
-val loc_of_cloc_of_loc (l: loc) : Lemma
-  (loc_of_cloc (cloc_of_loc l) == l)
-  [SMTPat (loc_of_cloc (cloc_of_loc l))]
 let loc_of_cloc_of_loc l = ()
 
-val cloc_of_loc_of_cloc (l: MG.loc cloc_cls) : Lemma
-  (cloc_of_loc (loc_of_cloc l) == l)
-  [SMTPat (cloc_of_loc (loc_of_cloc l))]
 let cloc_of_loc_of_cloc l = ()
 
-val cloc_of_loc_none: unit -> Lemma (cloc_of_loc loc_none == MG.loc_none)
 let cloc_of_loc_none _ = ()
 
-val cloc_of_loc_union (l1 l2: loc) : Lemma
-  (cloc_of_loc (loc_union l1 l2) == MG.loc_union (cloc_of_loc l1) (cloc_of_loc l2))
 let cloc_of_loc_union _ _ = ()
 
-val cloc_of_loc_addresses
-  (preserve_liveness: bool)
-  (r: HS.rid)
-  (n: Set.set nat)
-: Lemma
-  (cloc_of_loc (loc_addresses preserve_liveness r n) == MG.loc_addresses preserve_liveness r n)
 let cloc_of_loc_addresses _ _ _ = ()
 
-val cloc_of_loc_regions
-  (preserve_liveness: bool)
-  (r: Set.set HS.rid)
-: Lemma
-  (cloc_of_loc (loc_regions preserve_liveness r) == MG.loc_regions preserve_liveness r)
 let cloc_of_loc_regions _ _ = ()
 
-val loc_includes_to_cloc (l1 l2: loc) : Lemma
-  (loc_includes l1 l2 <==> MG.loc_includes (cloc_of_loc l1) (cloc_of_loc l2))
 let loc_includes_to_cloc l1 l2 = ()
 
-val loc_disjoint_to_cloc (l1 l2: loc) : Lemma
-  (loc_disjoint l1 l2 <==> MG.loc_disjoint (cloc_of_loc l1) (cloc_of_loc l2))
 let loc_disjoint_to_cloc l1 l2 = ()
 
-val modifies_to_cloc (l: loc) (h1 h2: HS.mem) : Lemma
-  (modifies l h1 h2 <==> MG.modifies (cloc_of_loc l) h1 h2)
 let modifies_to_cloc l h1 h2 = ()
